@base              <https://w3id.org/valueflows/ont/vf> .
@prefix vf:        <#> .
@prefix as:        <https://www.w3.org/ns/activitystreams#> .
@prefix cc:        <http://creativecommons.org/ns#> .
@prefix dcterms:   <http://purl.org/dc/terms/> .
@prefix dtype:     <http://www.linkedmodel.org/schema/dtype#> .
@prefix foaf:      <http://xmlns.com/foaf/0.1/> .
@prefix geo:       <http://www.w3.org/2003/01/geo/wgs84_pos#> .
@prefix geosparql: <http://www.opengis.net/ont/geosparql#> .
@prefix om:        <http://www.ontology-of-units-of-measure.org/resource/om-2/> .
@prefix org:       <http://www.w3.org/ns/org#> .
@prefix owl:       <http://www.w3.org/2002/07/owl#> .
@prefix rdf:       <http://www.w3.org/1999/02/22-rdf-syntax-ns#> .
@prefix rdfs:      <http://www.w3.org/2000/01/rdf-schema#> .
@prefix skos:      <http://www.w3.org/2004/02/skos/core#> .
@prefix spdxt:     <http://spdx.org/rdf/terms#> .
@prefix spdxl:     <https://spdx.org/licenses/> .
@prefix time:      <http://www.w3.org/2006/time#> .
@prefix vann:      <http://purl.org/vocab/vann/> .
@prefix vs:        <http://www.w3.org/2003/06/sw-vocab-status/ns#> .
@prefix xsd:       <http://www.w3.org/2001/XMLSchema#> .

<> a owl:Ontology ;
    dcterms:title "Valueflows Ontology" ;
    dcterms:description "A vocabulary for the distributed economic networks of the next economy, to coordinate the creation, distribution, and exchange of economic resources" ;
    dcterms:type <http://purl.org/adms/assettype/Ontology> ;
    vann:preferredNamespacePrefix "vf" ;
    vann:preferredNamespaceUri "https://w3id.org/valueflows/ont/vf#" ;
    owl:versionInfo "0.13" ;
    owl:versionIRI <https://w3id.org/valueflows/ont/0.13/vf> ;
    dcterms:status <http://purl.org/adms/status/UnderDevelopment> ;
    dcterms:license "https://creativecommons.org/licenses/by-sa/4.0/" ;
    cc:license "https://creativecommons.org/licenses/by-sa/4.0/" ;
    spdxt:licenseDeclared spdxl:CC-BY-SA-4.0 ;
    dcterms:source "https://codeberg.org/valueflows/pages/src/branch/main/assets/all_vf.TTL" ;
    .


#################################################################
#    Classes
#################################################################

# KNOWLEDGE LAYER CLASSES

vf:ResourceSpecification a  owl:Class ;
        rdfs:label          "Resource Specification"@en ;
        vs:term_status      "stable" ;
        rdfs:comment        "Specifies the kind of resource, even if the resource is not instantiated as an EconomicResource. Could define a material item, service, digital item, currency account, skill or type of work, etc."@en ;
        .

vf:ProcessSpecification a   owl:Class ;
        rdfs:label          "Process Specification"@en ;
        vs:term_status      "stable" ;
        rdfs:comment        "Specifies the kind of process."@en ;
        .

vf:Action  a                owl:Class ;
        rdfs:label          "Action"@en ;
        vs:term_status      "stable" ;
        rdfs:comment        "An action verb defining the kind of flow and its behavior."@en ;
        .

vf:InputOutput a            owl:Class ;
        rdfs:label          "Input/Output"@en ;
        vs:term_status      "testing" ;
        rdfs:comment        "The action is an input or output of a process, or not related to a process."@en ;
        .

vf:CreateResource a         owl:Class ;
        rdfs:label          "Create Resource"@en ;
        vs:term_status      "testing" ;
        rdfs:comment        "The action can create an economic resource."@en ;
        .

vf:EventQuantity a          owl:Class ;
        rdfs:label          "Event Quantity"@en ;
        vs:term_status      "testing" ;
        rdfs:comment        "The action involves the event resource quantity, event quantity, or both."@en ;
        .

vf:AccountingEffect a        owl:Class ;
        rdfs:label          "Accounting Effect"@en ;
        vs:term_status      "testing" ;
        rdfs:comment        "The action has this effect on an inventoried resource accounting quantity."@en ;
        .

vf:OnhandEffect a           owl:Class ;
        rdfs:label          "Onhand Effect"@en ;
        vs:term_status      "testing" ;
        rdfs:comment        "The action has this effect on an inventoried resource onhand quantity."@en ;
        .

vf:LocationEffect a         owl:Class ;
        rdfs:label          "Location Effect"@en ;
        vs:term_status      "testing" ;
        rdfs:comment        "The action has this effect on an inventoried resource current location."@en ;
        .

vf:ContainedEffect a        owl:Class ;
        rdfs:label          "Contained Effect"@en ;
        vs:term_status      "testing" ;
        rdfs:comment        "The action has this effect on an inventoried resource contained in resource."@en ;
        .

vf:AccountableEffect a      owl:Class ;
        rdfs:label          "Accountable Effect"@en ;
        vs:term_status      "testing" ;
        rdfs:comment        "The action has this effect on an inventoried resource primary accountable agent."@en ;
        .

vf:StageEffect a            owl:Class ;
        rdfs:label          "Stage Effect"@en ;
        vs:term_status      "testing" ;
        rdfs:comment        "The action has this effect on an inventoried resource stage."@en ;
        .

vf:StateEffect a            owl:Class ;
        rdfs:label          "State Effect"@en ;
        vs:term_status      "unstable" ;
        rdfs:comment        "The action has this effect on an inventoried resource state."@en ;
        .

vf:AgentRelationshipRole  a  owl:Class ;
        rdfs:label           "Agent Relationship Role"@en ;
        vs:term_status       "stable" ;
        rdfs:comment         "A relationship role defining the kind of association one agent can have with another."@en ;
        .

vf:Recipe a                 owl:Class ;
        rdfs:label          "Recipe"@en ;
        vs:term_status      "testing" ;
        rdfs:comment        "Optional instance of a recipe which directly specifies the recipe processes included."@en ;
        .

vf:RecipeGroup a            owl:Class ;
        rdfs:label          "Recipe Group"@en ;
        vs:term_status      "testing" ;
        rdfs:comment        "A grouping of recipes to facilitate planning them together."@en ;
        .

vf:RecipeProcess a          owl:Class ;
        rdfs:label          "Recipe Process"@en ;
        vs:term_status      "stable" ;
        rdfs:comment        "Specifies a process in a recipe for use in planning from recipe."@en ;
        .

vf:RecipeFlow a             owl:Class ;
        rdfs:label          "Recipe Flow"@en ;
        vs:term_status      "stable" ;
        rdfs:comment        "The specification of a resource inflow to, or outflow from, a recipe process."@en ;
        .

vf:RecipeExchange a         owl:Class ;
        rdfs:label          "Recipe Exchange"@en ;
        vs:term_status      "stable" ;
        rdfs:comment        "Specifies an exchange type agreement as part of a recipe."@en ;
        .

vf:ScenarioDefinition a     owl:Class ;
        rdfs:label          "Scenario Definition"@en ;
        vs:term_status      "unstable" ;
        rdfs:comment        "The type definition of one or more scenarios."@en ;
        .


# PLANNING LAYER CLASSES

vf:Plan  a                  owl:Class ;
        rdfs:label          "Plan"@en ;
        vs:term_status      "stable" ;
        rdfs:comment        "A logical collection of processes that constitute a body of scheduled work with defined deliverable(s)."@en ;
        .

vf:Intent  a                owl:Class ;
        rdfs:label          "Intent"@en ;
        vs:term_status      "stable" ;
        rdfs:comment        "A proposed or planned or estimated economic flow, prior to a commitment or agreement, which can lead to commitments and/or economic events."@en ;
        .

vf:Proposal  a              owl:Class ;
        rdfs:label          "Proposal"@en ;
        vs:term_status      "stable" ;
        rdfs:comment        "Published requests or offers, sometimes with what is expected in return."@en ;
        .

vf:ProposalList  a          owl:Class ;
        rdfs:label          "Proposal List"@en ;
        vs:term_status      "unstable" ;
        rdfs:comment        "A grouping of proposals, for publishing as a list."@en ;
        .

vf:ProposalPurpose a        owl:Class ;
        rdfs:label          "Proposal Purpose"@en ;
        vs:term_status      "testing" ;
        rdfs:comment        "The type of proposal, an offer or request (others may be added)."@en ;
        .

vf:Commitment  a            owl:Class ;
        rdfs:label          "Commitment"@en ;
        vs:term_status      "stable" ;
        rdfs:comment        "A planned economic flow that has been promised by an agent to another agent."@en ;
        .

vf:Agreement  a             owl:Class ;
        rdfs:label          "Agreement"@en ;
        vs:term_status      "stable" ;
        rdfs:comment        "Any type of agreement among economic agents."@en ;
        .

vf:AgreementBundle  a       owl:Class ;
        rdfs:label          "Agreement Bundle"@en ;
        vs:term_status      "unstable" ;
        rdfs:comment        "A grouping of agreements to bundle detailed line item reciprocity."@en ;
        .

vf:Scenario  a              owl:Class ;
        rdfs:label          "Scenario"@en ;
        vs:term_status      "unstable" ;
        rdfs:comment        "An estimated or analytical logical collection of higher level processes used for budgeting, analysis, plan refinement, etc."@en ;
        .


# OBSERVATION LAYER CLASSES

vf:Agent  a                 owl:Class ;
        rdfs:seeAlso        foaf:Agent ;
        rdfs:label          "Agent"@en ;
        vs:term_status      "stable" ;
        rdfs:comment        "An entity that can commit to and/or perform economic and/or ecological activity under its own power or authority."@en ;
        .

vf:Person  a                owl:Class ;
        rdfs:seeAlso        foaf:Person ;
        rdfs:label          "Person"@en ;
        rdfs:subClassOf     vf:Agent ;
        vs:term_status      "stable" ;
        rdfs:comment        "A human being. All people are considered agents."@en ;
        .

vf:Organization  a          owl:Class ;
        rdfs:seeAlso        org:Organization ;
        rdfs:label          "Organization"@en ;
        rdfs:subClassOf     vf:Agent ;
        vs:term_status      "stable" ;
        rdfs:comment        "A functional structure, formal or informal, which can include people and/or other organizations, and has its own agency.  Something called a group is an Organization in Valueflows if it has its own agency."@en ;
        .

vf:EcologicalAgent  a       owl:Class ;
        rdfs:label          "Ecological Agent"@en ;
        rdfs:subClassOf     vf:Agent ;
        vs:term_status      "testing" ;
        rdfs:comment        "A non-human being; or a functional group of non-human beings; or an ecosystem of living beings that includes non-humans."@en ;
        .

vf:EconomicResource  a      owl:Class ;
        rdfs:label          "Economic Resource"@en ;
        vs:term_status      "stable" ;
        rdfs:comment        "Economic or environmental inputs to or outputs from processes."@en ;
        .

vf:Process  a               owl:Class ;
        rdfs:label          "Process"@en ;
        vs:term_status      "stable" ;
        rdfs:comment        "An activity that changes inputs into outputs, by transforming or transporting economic resource(s)."@en ;
        .

vf:EconomicEvent  a         owl:Class ;
        rdfs:label          "Economic Event"@en ;
        vs:term_status      "stable" ;
        rdfs:comment        "An observed economic flow, as opposed to a flow planned to happen in the future. This could reflect a change in the quantity of an economic resource. It is also defined by its behavior in relation to the economic resource (see vf:action)"@en ;
        .

vf:AgentRelationship  a     owl:Class ;
        rdfs:seeAlso        as:Relationship ;
        rdfs:label          "Agent Relationship"@en ;
        vs:term_status      "stable" ;
        rdfs:comment        "An ongoing voluntary association between 2 agents of any kind."@en ;
        .

vf:Claim  a                 owl:Class ;
        rdfs:label          "Claim"@en ;
        vs:term_status      "testing" ;
        rdfs:comment        "A claim for a future economic event(s) in reciprocity for an economic event that already occurred. For example, a claim for payment for goods received."@en ;
        .

# UTILITY CLASSES

vf:SpatialThing a           owl:Class ;
        rdfs:subClassOf     geo:SpatialThing ;
        rdfs:label          "Spatial Thing"@en ;
        vs:term_status      "stable" ;
        rdfs:comment        "Data that locates something relative to the Earth, usually a somewhat fixed location."@en ;
        .

vf:Measure a                owl:Class ;
        rdfs:subClassOf     om:Measure ;
        rdfs:label          "Measure"@en ;
        vs:term_status      "stable" ;
        rdfs:comment        "A quantity expressed as a numeric value with a unit of measure."@en ;
        .

vf:Unit a                   owl:Class ;
        rdfs:subClassOf     om:Unit ;
        rdfs:label          "Unit"@en ;
        vs:term_status      "stable" ;
        rdfs:comment        "A standard unit of measure, defined and adopted by convention or by law."@en ;
        .


#################################################################
#    Properties
#################################################################

vf:action
        a                   owl:ObjectProperty ;
        rdfs:label          "action"@en ;
        rdfs:domain         [ owl:unionOf (vf:EconomicEvent vf:Commitment vf:Intent vf:RecipeFlow vf:Claim) ] ;
        rdfs:range          vf:Action ;
        owl:cardinality     1 ;
        vs:term_status      "stable" ;
        rdfs:comment        "Defines the kind of flow, such as consume, produce, work, transfer, etc."@en ;
        .

vf:inputOf
        a                   owl:ObjectProperty ;
        rdfs:label          "input of"@en ;
        rdfs:domain         [ owl:unionOf (vf:EconomicEvent vf:Commitment vf:Intent) ] ;
        rdfs:range          vf:Process ;
        owl:maxCardinality  1 ;
        vs:term_status      "stable" ;
        rdfs:comment        "Relates an input flow to its process."@en ;
        .

vf:hasInput
        a                   owl:ObjectProperty ;
        owl:inverseOf       vf:inputOf ;
        rdfs:label          "has input"@en ;
        rdfs:domain         vf:Process ;
        rdfs:range          [ owl:unionOf (vf:EconomicEvent vf:Commitment vf:Intent) ] ;
        vs:term_status      "testing" ;
        rdfs:comment        "All the input flows of a process."@en ;
        .

vf:outputOf
        a                   owl:ObjectProperty ;
        rdfs:label          "output of"@en ;
        rdfs:domain         [ owl:unionOf (vf:EconomicEvent vf:Commitment vf:Intent) ] ;
        rdfs:range          vf:Process ;
        owl:maxCardinality  1 ;
        vs:term_status      "stable" ;
        rdfs:comment        "Relates an output flow to its process."@en ;
        .

vf:hasOutput
        a                   owl:ObjectProperty ;
        owl:inverseOf       vf:outputOf ;
        rdfs:label          "has output"@en ;
        rdfs:domain         vf:Process ;
        rdfs:range          [ owl:unionOf (vf:EconomicEvent vf:Commitment vf:Intent) ] ;
        vs:term_status      "testing" ;
        rdfs:comment        "All the output flows of a process."@en ;
        .

vf:recipeInputOf
        a                   owl:ObjectProperty ;
        rdfs:label          "recipe input of"@en ;
        rdfs:domain         vf:RecipeFlow ;
        rdfs:range          vf:RecipeProcess ;
        owl:maxCardinality  1 ;
        vs:term_status      "stable" ;
        rdfs:comment        "Relates an input flow to its process in a recipe."@en ;
        .

vf:hasRecipeInput
        a                   owl:ObjectProperty ;
        owl:inverseOf       vf:recipeInputOf ;
        rdfs:label          "has recipe input"@en ;
        rdfs:domain         vf:RecipeProcess ;
        rdfs:range          vf:RecipeFlow ;
        vs:term_status      "testing" ;
        rdfs:comment        "All the inputs of a recipe process."@en ;
        .

vf:recipeOutputOf
        a                   owl:ObjectProperty ;
        rdfs:label          "recipe output of"@en ;
        rdfs:domain         vf:RecipeFlow ;
        rdfs:range          vf:RecipeProcess ;
        owl:maxCardinality  1 ;
        vs:term_status      "stable" ;
        rdfs:comment        "Relates an output flow to its process in a recipe."@en ;
        .

vf:hasRecipeOutput
        a                   owl:ObjectProperty ;
        owl:inverseOf       vf:recipeOutputOf ;
        rdfs:label          "has recipe output"@en ;
        rdfs:domain         vf:RecipeProcess ;
        rdfs:range          vf:RecipeFlow ;
        vs:term_status      "testing" ;
        rdfs:comment        "All the outputs of a recipe process."@en ;
        .

vf:recipeClauseOf
        a                   owl:ObjectProperty ;
        rdfs:label          "recipe clause of"@en ;
        rdfs:domain         vf:RecipeFlow ;
        rdfs:range          vf:RecipeExchange ;
        owl:maxCardinality  1 ;
        vs:term_status      "stable" ;
        rdfs:comment        "Relates a flow to its exchange agreement in a recipe."@en ;
        .

vf:recipeStipulates
        a                   owl:ObjectProperty ;
        owl:inverseOf       vf:recipeClauseOf ;
        rdfs:label          "recipe stipulates"@en ;
        rdfs:domain         vf:RecipeExchange ;
        rdfs:range          vf:RecipeFlow ;
        vs:term_status      "testing" ;
        rdfs:comment        "All the primary clauses of a recipe exchange."@en ;
        .

vf:recipeReciprocalClauseOf
        a                   owl:ObjectProperty ;
        rdfs:label          "recipe reciprocal clause of"@en ;
        rdfs:domain         vf:RecipeFlow ;
        rdfs:range          vf:RecipeExchange ;
        owl:maxCardinality  1 ;
        vs:term_status      "stable" ;
        rdfs:comment        "Relates a reciprocal flow to its exchange agreement in a recipe."@en ;
        .

vf:recipeStipulatesReciprocal
        a                   owl:ObjectProperty ;
        owl:inverseOf       vf:recipeReciprocalClauseOf ;
        rdfs:label          "recipe stipulates reciprocal"@en ;
        rdfs:domain         vf:RecipeExchange ;
        rdfs:range          vf:RecipeFlow ;
        vs:term_status      "testing" ;
        rdfs:comment        "All the reciprocal clauses of a recipe exchange."@en ;
        .

vf:plannedTogether
        a                   owl:ObjectProperty ;
        rdfs:label          "planned together"@en ;
        rdfs:domain         vf:RecipeGroup ;
        rdfs:range          vf:Recipe ;
        vs:term_status      "unstable" ;
        rdfs:comment        "A collection of recipes that can be planned together."@en ;
        .

vf:primaryOutput
        a                   owl:ObjectProperty ;
        rdfs:label          "primary output"@en ;
        rdfs:domain         vf:Recipe ;
        rdfs:range          vf:ResourceSpecification ;
        owl:maxCardinality  1 ;
        vs:term_status      "unstable" ;
        rdfs:comment        "The main output the recipe is intended to produce or deliver."@en ;
        .

vf:recipeIncludes
        a                   owl:ObjectProperty ;
        rdfs:label          "recipe includes"@en ;
        rdfs:domain         vf:Recipe ;
        rdfs:range          vf:RecipeProcess ;
        vs:term_status      "unstable" ;
        rdfs:comment        "The collection of processes needed for this recipe."@en ;
        .

vf:plannedWithin
        a                   owl:ObjectProperty ;
        rdfs:label          "planned within"@en ;
        rdfs:domain         [ owl:unionOf (vf:Process vf:Commitment vf:Intent) ] ;
        rdfs:range          vf:Plan ;
        owl:maxCardinality  1 ;
        vs:term_status      "testing" ;
        rdfs:comment        "The non-process commitment/intent or process with its inputs and outputs is part of the plan."@en ;
        .

vf:planIncludes
        a                   owl:ObjectProperty ;
        owl:inverseOf       vf:plannedWithin ;
        rdfs:label          "plan includes"@en ;
        rdfs:domain         vf:Plan ;
        rdfs:range          [ owl:unionOf (vf:Process vf:Commitment vf:Intent) ] ;
        vs:term_status      "testing" ;
        rdfs:comment        "The processes and and non-process commitments/intents that constitute the plan."@en ;
        .

vf:independentDemandOf
        a                   owl:ObjectProperty ;
        rdfs:label          "independent demand of"@en ;
        rdfs:range          vf:Plan ;
        rdfs:domain         [ owl:unionOf (vf:Commitment vf:Intent) ] ;
        owl:maxCardinality  1 ;
        vs:term_status      "testing" ;
        rdfs:comment        "This plan is the way this commitment or intent will be realized."@en ;
        .

vf:hasIndependentDemand
        a                   owl:ObjectProperty ;
        owl:inverseOf       vf:independentDemandOf ;
        rdfs:label          "has independent demand"@en ;
        rdfs:range          [ owl:unionOf (vf:Commitment vf:Intent) ]  ;
        rdfs:domain         vf:Plan ;
        vs:term_status      "testing" ;
        rdfs:comment        "The commitments and/or intents which this plan was created to deliver."@en ;
        .

vf:resourceInventoriedAs
        a                   owl:ObjectProperty ;
        rdfs:label          "resource inventoried as"@en ;
        rdfs:domain         [ owl:unionOf (vf:Commitment vf:Intent vf:EconomicEvent) ] ;
        rdfs:range          vf:EconomicResource ;
        owl:maxCardinality  1 ;
        vs:term_status      "stable" ;
        rdfs:comment        "Economic resource involved in the flow."@en ;
        .

vf:toResourceInventoriedAs
        a                   owl:ObjectProperty ;
        rdfs:label          "to resource inventoried as"@en ;
        rdfs:domain         vf:EconomicEvent ;
        rdfs:range          vf:EconomicResource ;
        owl:maxCardinality  1 ;
        vs:term_status      "stable" ;
        rdfs:comment        "Additional economic resource on the economic event when needed by the receiver. Used when a transfer or move, or sometimes other actions, requires explicitly identifying an economic resource on the receiving side."@en ;
        .

vf:provider  a              owl:ObjectProperty ;
        rdfs:domain         [ owl:unionOf (vf:EconomicEvent vf:Commitment vf:Intent vf:Claim) ] ;
        rdfs:label          "provider"@en ;
        rdfs:range          vf:Agent ;
        owl:maxCardinality  1 ;
        vs:term_status      "stable" ;
        rdfs:comment        "The economic agent from whom the intended, committed, or actual economic event is initiated."@en ;
        .

vf:receiver  a              owl:ObjectProperty ;
        rdfs:domain         [ owl:unionOf (vf:EconomicEvent vf:Commitment vf:Intent vf:Claim) ] ;
        rdfs:label          "receiver"@en ;
        rdfs:range          vf:Agent ;
        owl:maxCardinality  1 ;
        vs:term_status      "stable" ;
        rdfs:comment        "The economic agent whom the intended, committed, or actual economic event is for."@en ;
        .

vf:subject  a               owl:ObjectProperty ;
        rdfs:seeAlso        as:subject ;
        rdfs:domain         vf:AgentRelationship ;
        rdfs:label          "subject"@en ;
        rdfs:range          vf:Agent ;
        owl:cardinality     1 ;
        vs:term_status      "stable" ;
        rdfs:comment        "The subject of a relationship between 2 agents.  For example, if Mary is a member of a group, then Mary is the subject."@en ;
        .

vf:object  a                owl:ObjectProperty ;
        rdfs:seeAlso        as:object ;
        rdfs:domain         vf:AgentRelationship ;
        rdfs:label          "object"@en ;
        rdfs:range          vf:Agent ;
        owl:cardinality     1 ;
        vs:term_status      "stable" ;
        rdfs:comment        "The object of a relationship between 2 agents.  For example, if Mary is a member of a group, then the group is the object."@en ;
        .

vf:relationship  a          owl:ObjectProperty ;
        rdfs:seeAlso        as:relationship ;
        rdfs:label          "relationship"@en ;
        rdfs:domain         vf:AgentRelationship ;
        rdfs:range          vf:AgentRelationshipRole ;
        owl:cardinality     1 ;
        vs:term_status      "stable" ;
        rdfs:comment        "The role of an economic relationship that exists between 2 agents, such as member, trading partner."@en ;
        .

vf:inScopeOf  a             owl:ObjectProperty ;
        rdfs:domain         [ owl:unionOf (vf:Claim vf:Commitment vf:EconomicEvent vf:Proposal vf:Intent vf:Scenario vf:Process vf:AgentRelationship) ] ;
        rdfs:label          "in scope of"@en ;
        rdfs:range          vf:Agent ;
        owl:maxCardinality  1 ;
        vs:term_status      "testing" ;
        rdfs:comment        "In the context of an agent, a grouping generally used for accounting, reporting."@en ;
        .

vf:triggeredBy  a           owl:ObjectProperty ;
        rdfs:label          "triggered by"@en ;
        rdfs:domain         vf:Claim ;
        rdfs:range          vf:EconomicEvent ;
        owl:maxCardinality  1 ;
        vs:term_status      "testing" ;
        rdfs:comment        "References an economic event that implied the claim, often based on a prior agreement."@en ;
        .

vf:corrects  a              owl:ObjectProperty ;
        rdfs:label          "corrects"@en ;
        rdfs:domain         vf:EconomicEvent ;
        rdfs:range          vf:EconomicEvent ;
        owl:maxCardinality  1 ;
        vs:term_status      "unstable" ;
        rdfs:comment        "Used when an event was entered incorrectly and needs to be backed out or corrected. (The initial event cannot be changed.)"@en ;
        .

vf:settles  a               owl:ObjectProperty ;
        rdfs:label          "settles"@en ;
        rdfs:domain         vf:EconomicEvent ;
        rdfs:range          vf:Claim ;
        vs:term_status      "testing" ;
        rdfs:comment        "References a claim that is fully or partially settled by the economic event."@en ;
        .

vf:containedIn a            owl:ObjectProperty ;
        rdfs:label          "contained in"@en ;
        rdfs:domain         vf:EconomicResource ;
        rdfs:range          vf:EconomicResource ;
        owl:maxCardinality  1 ;
        vs:term_status      "unstable" ;
        rdfs:comment        "Used when a stock economic resource contains units also defined as economic resources."@en ;
        .

vf:primaryAccountable a     owl:ObjectProperty ;
        rdfs:label          "primary accountable"@en ;
        rdfs:domain         vf:EconomicResource ;
        rdfs:range          vf:Agent ;
        owl:maxCardinality  1 ;
        vs:term_status      "stable" ;
        rdfs:comment        "The agent currently with primary rights and responsibilites for the economic resource. It is the agent that is associated with the accountingQuantity of the economic resource."@en ;
        .

vf:hasBeginning a           owl:DatatypeProperty ;
        rdfs:subPropertyOf  time:hasBeginning ;
        rdfs:label          "has beginning"@en ;
        rdfs:domain         [ owl:unionOf (
                                vf:Commitment
                                vf:EconomicEvent
                                vf:Intent
                                vf:Proposal
                                vf:Scenario
                                vf:Process) ] ;
        rdfs:range          xsd:dateTimeStamp ;
        owl:maxCardinality  1 ;
        vs:term_status      "stable" ;
        rdfs:comment        "The planned or actual beginning of a flow or process."@en ;
        .

vf:hasEnd a                 owl:DatatypeProperty ;
        rdfs:subPropertyOf  time:hasEnd ;
        rdfs:label          "has end"@en ;
        rdfs:domain         [ owl:unionOf (
                                vf:Commitment
                                vf:EconomicEvent
                                vf:Intent
                                vf:Proposal
                                vf:Scenario
                                vf:Process) ] ;
        rdfs:range          xsd:dateTimeStamp ;
        owl:maxCardinality  1 ;
        vs:term_status      "stable" ;
        rdfs:comment        "The planned or actual end of a flow or process."@en ;
        .

vf:hasPointInTime a         owl:DatatypeProperty ;
        rdfs:subPropertyOf  time:inXSDDateTimeStamp ;
        rdfs:label          "has point in time"@en ;
        rdfs:domain         [ owl:unionOf (
                                vf:Commitment
                                vf:EconomicEvent
                                vf:Intent) ] ;
        rdfs:range          xsd:dateTimeStamp ;
        owl:maxCardinality  1 ;
        vs:term_status      "stable" ;
        rdfs:comment        "The planned or actual time of a flow; can be used instead of hasBeginning and hasEnd, if so, hasBeginning and hasEnd should be able to be returned with this value."@en ;
        .

vf:hasDuration a            owl:ObjectProperty ;
        rdfs:seeAlso        time:hasDuration ;
        rdfs:label          "has duration"@en ;
        rdfs:domain         [ owl:unionOf (
                                vf:RecipeProcess
                                vf:ScenarioDefinition) ] ;
        rdfs:range          vf:Measure ;
        owl:maxCardinality  1 ;
        vs:term_status      "testing" ;
        rdfs:comment        "The temporal extent of the process or scenario."@en ;
        .

vf:due a                    owl:DatatypeProperty ;
        rdfs:label          "due"@en ;
        rdfs:domain         [ owl:unionOf (
                                vf:Plan
                                vf:Commitment
                                vf:Claim
                                vf:Intent) ] ;
        rdfs:range          xsd:dateTimeStamp ;
        owl:maxCardinality  1 ;
        vs:term_status      "stable" ;
        rdfs:comment        "The time something is expected to be complete."@en ;
        .

vf:hasNumericalValue a      owl:DatatypeProperty ;
        rdfs:subPropertyOf  om:hasNumericalValue ;
        rdfs:label          "has numerical value"@en ;
        rdfs:domain         vf:Measure ;
        rdfs:range          dtype:numericUnion ;
        owl:maxCardinality  1 ;
        vs:term_status      "stable" ;
        rdfs:comment        "A numeric amount."@en ;
        .

vf:hasUnit a                owl:ObjectProperty ;
        rdfs:subPropertyOf  om:hasUnit ;
        rdfs:label          "has unit"@en ;
        rdfs:domain         vf:Measure ;
        rdfs:range          vf:Unit ;
        owl:maxCardinality  1 ;
        vs:term_status      "stable" ;
        rdfs:comment        "A standard unit of measure."@en ;
        .

vf:omUnitIdentifier a       owl:DataTypeProperty ;
        rdfs:label          "om unit identifier"@en ;
        rdfs:domain         vf:Unit ;
        rdfs:range          xsd:anyURI ;
        owl:maxCardinality  1 ;
        vs:term_status      "testing" ;
        rdfs:comment        "The unique identifier of the om unit of measure, for standardization across networks."@en ;
        .

vf:label a                  owl:DataTypeProperty ;
        rdfs:subPropertyOf  rdfs:label ;
        rdfs:label          "label"@en ;
        rdfs:domain         [ owl:unionOf (
                                vf:Unit
                                vf:Action) ] ;
        rdfs:range          xsd:string ;
        owl:cardinality     1 ;
        vs:term_status      "stable" ;
        rdfs:comment        "The display label defined in om for the unit of measure."@en ;
        .

vf:symbol a                 owl:DataTypeProperty ;
        rdfs:subPropertyOf  om:symbol ;
        rdfs:label          "symbol"@en ;
        rdfs:domain         vf:Unit ;
        rdfs:range          xsd:string ;
        owl:maxCardinality  1 ;
        vs:term_status      "testing" ;
        rdfs:comment        "The display symbol defined in om for the unit of measure."@en ;
        .

vf:overrideLabel a          owl:DataTypeProperty ;
        rdfs:label          "override label"@en ;
        rdfs:domain         vf:Unit ;
        rdfs:range          xsd:string ;
        owl:maxCardinality  1 ;
        vs:term_status      "testing" ;
        rdfs:comment        "An optional network override label to display for units of measure if the original is less appropriate."@en ;
        .

vf:overrideSymbol a         owl:DataTypeProperty ;
        rdfs:label          "override symbol"@en ;
        rdfs:domain         vf:Unit ;
        rdfs:range          xsd:string ;
        owl:maxCardinality  1 ;
        vs:term_status      "testing" ;
        rdfs:comment        "An optional network override symbol to display for units of measure if the original is less appropriate."@en ;
        .

vf:accountingQuantity a     owl:ObjectProperty ;
        rdfs:label          "accounting quantity"@en ;
        rdfs:domain         vf:EconomicResource ;
        rdfs:range          vf:Measure ;
        owl:maxCardinality  1 ;
        vs:term_status      "stable" ;
        rdfs:comment        "The current amount and unit of the economic resource for which the agent has primary rights and responsibilities, sometimes thought of as ownership. This can be either stored or derived from economic events affecting the resource."@en ;
        .

vf:onhandQuantity a         owl:ObjectProperty ;
        rdfs:label          "onhand quantity"@en ;
        rdfs:domain         vf:EconomicResource ;
        rdfs:range          vf:Measure ;
        owl:maxCardinality  1 ;
        vs:term_status      "testing" ;
        rdfs:comment        "The current amount and unit of the economic resource which is under direct control of the agent.  It may be more or less than the accounting quantity. This can be either stored or derived from economic events affecting the resource."@en ;
        .

vf:resourceQuantity a       owl:ObjectProperty ;
        rdfs:label          "resource quantity"@en ;
        rdfs:domain         [ owl:unionOf (vf:EconomicEvent vf:Commitment vf:Intent vf:RecipeFlow vf:Claim) ] ;
        rdfs:range          vf:Measure ;
        owl:maxCardinality  1 ;
        vs:term_status      "stable" ;
        rdfs:comment        "The amount and unit of the economic resource counted or inventoried."@en ;
        .

vf:effortQuantity a         owl:ObjectProperty ;
        rdfs:label          "effort quantity"@en ;
        rdfs:domain         [ owl:unionOf (vf:EconomicEvent vf:Commitment vf:Intent vf:RecipeFlow vf:Claim) ] ;
        rdfs:range          vf:Measure ;
        owl:maxCardinality  1 ;
        vs:term_status      "stable" ;
        rdfs:comment        "The amount and unit of the work or use or citation effort-based action. This is often expressed with a time unit, but also could be cycle counts or other measures of effort or usefulness."@en ;
        .

vf:availableQuantity a      owl:ObjectProperty ;
        rdfs:label          "available quantity"@en ;
        rdfs:domain         vf:Intent ;
        rdfs:range          vf:Measure ;
        owl:maxCardinality  1 ;
        vs:term_status      "stable" ;
        rdfs:comment        "The amount and unit of the offered resource currently available."@en ;
        .

vf:minimumQuantity a        owl:ObjectProperty ;
        rdfs:label          "minimum quantity"@en ;
        rdfs:domain         vf:Intent ;
        rdfs:range          vf:Measure ;
        owl:maxCardinality  1 ;
        vs:term_status      "testing" ;
        rdfs:comment        "The minimum required order amount and unit of the offered resource."@en ;
        .

vf:unitBased  a             owl:DatatypeProperty ;
        rdfs:label          "unit based"@en ;
        rdfs:domain         vf:Proposal ;
        rdfs:range          xsd:boolean ;
        owl:maxCardinality  1 ;
        vs:term_status      "stable" ;
        rdfs:comment        "This proposal contains unit based quantities, which can be multipied to create commitments; commonly seen in a price list or e-commerce. Default false."@en ;
        .

vf:purpose  a               owl:ObjectProperty ;
        rdfs:label          "purpose"@en ;
        rdfs:domain         vf:Proposal ;
        rdfs:range          vf:ProposalPurpose ;
        owl:maxCardinality  1 ;
        vs:term_status      "testing" ;
        rdfs:comment        "The type of proposal, offer or request."@en ;
        .

vf:created a                owl:DatatypeProperty ;
        rdfs:seeAlso        dcterms:created ;
        rdfs:label          "created"@en ;
        rdfs:domain         [ owl:unionOf (
                                vf:Agreement
                                vf:Claim
                                vf:Commitment
                                vf:Plan
                                vf:Proposal
                                vf:Scenario
                                vf:EconomicEvent ) ] ;
        rdfs:range          xsd:dateTimeStamp ;
        owl:maxCardinality  1 ;
        vs:term_status      "testing" ;
        rdfs:comment        "The date, and time if desired, the information was agreed to or recorded."@en ;
        .

vf:long a                   owl:DatatypeProperty ;
        rdfs:subPropertyOf  geo:long ;
        rdfs:range          dtype:numericUnion ;
        rdfs:domain         vf:SpatialThing ;
        owl:maxCardinality  1 ;
        vs:term_status      "testing" ;
        rdfs:comment        "The WGS84 longitude of a spatial thing (decimal degrees)." ;
        .

vf:lat a                    owl:DatatypeProperty ;
        rdfs:subPropertyOf  geo:lat ;
        rdfs:range          dtype:numericUnion ;
        rdfs:domain         vf:SpatialThing ;
        owl:maxCardinality  1 ;
        vs:term_status      "testing" ;
        rdfs:comment        "The WGS84 latitude of a spatial thing (decimal degrees)." ;
        .

vf:alt a                    owl:DatatypeProperty ;
        rdfs:subPropertyOf  geo:alt ;
        rdfs:range          dtype:numericUnion ;
        rdfs:domain         vf:SpatialThing ;
        owl:maxCardinality  1 ;
        vs:term_status      "testing" ;
        rdfs:comment        "The WGS84 altitude of a spatial thing (decimal meters above the local reference ellipsoid)" ;
        .

vf:mappableAddress a        owl:DatatypeProperty ;
        rdfs:label          "mappable address"@en ;
        rdfs:domain         vf:SpatialThing ;
        rdfs:range          xsd:string ;
        owl:maxCardinality  1 ;
        vs:term_status      "testing" ;
        rdfs:comment        "A textual address that can be mapped using mapping software."@en ;
        .

vf:hasDetailedGeometry a    owl:ObjectProperty ;
        rdfs:label          "currency address"@en ;
        rdfs:domain         vf:SpatialThing ;
        rdfs:range          geosparql:Geometry ;
        vs:term_status      "unstable" ;
        rdfs:comment        "A spatial geometry of any complexity and tooling supported by geosparql."@en ;
        .

vf:currentLocation a        owl:ObjectProperty ;
        rdfs:label          "current location"@en ;
        rdfs:domain         vf:EconomicResource ;
        rdfs:range          vf:SpatialThing ;
        owl:maxCardinality  1 ;
        vs:term_status      "stable" ;
        rdfs:comment        "The current physical location of an economic resource.  Could be at any level of granularity, from a town to an address to a warehouse location.  Usually mappable."@en ;
        .

vf:currentVirtualLocation
        a                   owl:DatatypeProperty ;
        rdfs:label          "current virtual location"@en ;
        rdfs:domain         vf:EconomicResource ;
        rdfs:range          xsd:anyURI ;
        owl:maxCardinality  1 ;
        vs:term_status      "testing" ;
        rdfs:comment        "The current virtual place a digital economic resource is located. Usually used for documents, code, or other electronic resource."@en ;
        .

vf:currentCurrencyLocation
        a                   owl:DatatypeProperty ;
        rdfs:label          "current currency location"@en ;
        rdfs:domain         vf:EconomicResource ;
        rdfs:range          xsd:string ;
        owl:maxCardinality  1 ;
        vs:term_status      "unstable" ;
        rdfs:comment        "The current virtual place a currency economic resource is located, for example the address for a bank account, crypto wallet, etc., in a domain standard format."@en ;
        .

vf:primaryLocation a        owl:ObjectProperty ;
        rdfs:label          "primary location"@en ;
        rdfs:domain         vf:Agent ;
        rdfs:range          vf:SpatialThing ;
        owl:maxCardinality  1 ;
        vs:term_status      "testing" ;
        rdfs:comment        "The main place an agent is located, often an address where activities occur and mail can be sent. This is usually a mappable geographic location."@en ;
        .

vf:eligibleLocation a       owl:ObjectProperty ;
        rdfs:label          "eligible location"@en ;
        rdfs:domain         vf:Proposal ;
        rdfs:range          vf:SpatialThing ;
        owl:maxCardinality  1 ;
        vs:term_status      "unstable" ;
        rdfs:comment        "Location or area where the proposal is valid."@en ;
        .

vf:atLocation a             owl:ObjectProperty ;
        rdfs:label          "at location"@en ;
        rdfs:domain         [ owl:unionOf (vf:EconomicEvent vf:Commitment vf:Intent) ] ;
        rdfs:range          vf:SpatialThing ;
        owl:maxCardinality  1 ;
        vs:term_status      "unstable" ;
        rdfs:comment        "The place where an intent, commitment, or economic event occurs.  Usually mappable."@en ;
        .

vf:toLocation a             owl:ObjectProperty ;
        rdfs:label          "to location"@en ;
        rdfs:domain         vf:EconomicEvent ;
        rdfs:range          vf:SpatialThing ;
        owl:maxCardinality  1 ;
        vs:term_status      "unstable" ;
        rdfs:comment        "The new location of the receiver resource."@en ;
        .

vf:image a                  owl:DatatypeProperty ;
        rdfs:label          "image"@en ;
        rdfs:domain         [ owl:unionOf (
                                vf:Agent
                                vf:EconomicEvent
                                vf:EconomicResource
                                vf:Intent
                                vf:ResourceSpecification
                                vf:ProcessSpecification
                                vf:RecipeProcess) ] ;
        rdfs:range          xsd:anyURI ;
        owl:maxCardinality  1 ;
        vs:term_status      "stable" ;
        rdfs:comment        "The uri to an image relevant to the entity, such as a logo, avatar, photo, diagram, etc."@en ;
        .

vf:imageList a              owl:DatatypeProperty ;
        rdfs:label          "image list"@en ;
        rdfs:domain         [ owl:unionOf (
                                vf:EconomicResource
                                vf:Intent
                                vf:ResourceSpecification) ] ;
        rdfs:range          xsd:anyURI ;
        vs:term_status      "stable" ;
        rdfs:comment        "A comma separated list of uri addresses to images relevant to the resource."@en ;
        .

vf:name a                   owl:DatatypeProperty ;
        rdfs:label          "name"@en ;
        rdfs:range          xsd:string ;
        rdfs:domain         [ owl:unionOf (
                                vf:SpatialThing
                                vf:Agent
                                vf:Agreement
                                vf:EconomicResource
                                vf:Plan
                                vf:Process
                                vf:ProcessSpecification
                                vf:Proposal
                                vf:Recipe
                                vf:RecipeGroup
                                vf:RecipeProcess
                                vf:ResourceSpecification
                                vf:Scenario
                                vf:ScenarioDefinition) ] ;
        owl:maxCardinality  1 ;
        vs:term_status      "stable" ;
        rdfs:comment        "An informal or formal textual identifier for an object. Does not imply uniqueness."@en ;
        .

vf:note a                   owl:DataTypeProperty ;
        rdfs:subPropertyOf  skos:note ;
        rdfs:label          "note"@en ;
        rdfs:domain         [ owl:unionOf (
                                vf:Agent
                                vf:AgentRelationship
                                vf:AgentRelationshipRole
                                vf:Agreement
                                vf:Claim
                                vf:Commitment
                                vf:EconomicEvent
                                vf:EconomicResource
                                vf:ExternalLink
                                vf:Intent
                                vf:Plan
                                vf:Process
                                vf:ProcessSpecification
                                vf:Proposal
                                vf:Recipe
                                vf:RecipeFlow
                                vf:RecipeGroup
                                vf:RecipeProcess
                                vf:ResourceSpecification
                                vf:Scenario
                                vf:ScenarioDefinition
                                vf:SpatialThing) ] ;
        rdfs:range          xsd:string ;
        owl:maxCardinality  1 ;
        vs:term_status      "stable" ;
        rdfs:comment        "Any useful textual information related to the item."@en ;
        .

vf:trackingIdentifier a     owl:DatatypeProperty ;
        rdfs:label          "tracking identifier"@en ;
        rdfs:domain         vf:EconomicResource ;
        rdfs:range          xsd:string ;
        owl:maxCardinality  1 ;
        vs:term_status      "stable" ;
        rdfs:comment        "Any identifier used to track the resource, such as a serial number or VIN or lot/batch identifier."@en ;
        .

vf:fulfills  a              owl:ObjectProperty ;
        rdfs:label          "fulfills"@en ;
        rdfs:domain         vf:EconomicEvent ;
        rdfs:range          vf:Commitment ;
        vs:term_status      "testing" ;
        rdfs:comment        "The commitment which is completely or partially fulfilled by an economic event."@en ;
        .

vf:satisfies
        a                   owl:ObjectProperty ;
        rdfs:label          "satisfies"@en ;
        rdfs:domain         [ owl:unionOf (vf:Commitment vf:EconomicEvent ) ] ;
        rdfs:range          vf:Intent ;
        vs:term_status      "testing" ;
        rdfs:comment        "An intent satisfied fully or partially by an economic event or commitment."@en ;
        .

vf:publishes
        a                   owl:ObjectProperty ;
        rdfs:label          "publishes"@en ;
        rdfs:domain         vf:Proposal ;
        rdfs:range          vf:Intent ;
        vs:term_status      "testing" ;
        rdfs:comment        "The primary intent(s) of this published proposal. Would be used in intent matching."@en ;
        .

vf:reciprocal
        a                   owl:ObjectProperty ;
        rdfs:label          "reciprocal"@en ;
        rdfs:domain         vf:Proposal ;
        rdfs:range          vf:Intent ;
        vs:term_status      "testing" ;
        rdfs:comment        "The reciprocal intent(s) of this published proposal. Not meant to be used for intent matching."@en ;
        .

vf:publishedTo
        a                   owl:ObjectProperty ;
        rdfs:label          "published to"@en ;
        rdfs:domain         vf:Scenario  ;
        rdfs:range          vf:Agent ;
        vs:term_status      "unstable" ;
        rdfs:comment        "The agent(s) to which the scenario is published."@en ;
        .

vf:proposedTo
        a                   owl:ObjectProperty ;
        rdfs:label          "proposed to"@en ;
        rdfs:domain         [ owl:unionOf (vf:Proposal vf:ProposalList) ]  ;
        rdfs:range          vf:Agent ;
        vs:term_status      "unstable" ;
        rdfs:comment        "The agent(s) to which the proposal or proposal list is published."@en ;
        .

vf:listedIn a               owl:ObjectProperty ;
        rdfs:label          "listed in"@en ;
        rdfs:domain         vf:Proposal ;
        rdfs:range          vf:ProposalList ;
        vs:term_status      "testing" ;
        rdfs:comment        "This proposal is part of a list of proposals."@en ;
        .

vf:lists a                  owl:ObjectProperty ;
        owl:inverseOf       vf:listedIn ;
        rdfs:label          "lists"@en ;
        rdfs:domain         vf:ProposalList ;
        rdfs:range          vf:Proposal ;
        vs:term_status      "unstable" ;
        rdfs:comment        "All the proposals included in this proposal list."@en ;
        .

vf:finished  a              owl:DatatypeProperty ;
        rdfs:domain         [ owl:unionOf (vf:Commitment vf:Process vf:Intent vf:Claim) ] ;
        rdfs:label          "finished"@en ;
        rdfs:range          xsd:boolean ;
        owl:maxCardinality  1 ;
        vs:term_status      "stable" ;
        rdfs:comment        "The commitment or intent or process is complete or not.  This is irrespective of if the original goal has been met, and indicates that no more will be done.  Default false."@en ;
        .

vf:substitutable a          owl:DatatypeProperty ;
        rdfs:label          "substitutable"@en ;
        rdfs:domain         vf:ResourceSpecification ;
        rdfs:range          xsd:boolean ;
        owl:maxCardinality  1 ;
        vs:term_status      "stable" ;
        rdfs:comment        "Defines if any resource of that type can be freely substituted for any other resource of that type when used, consumed, traded, etc."@en ;
        .

vf:unitOfEffort a           owl:ObjectProperty ;
        rdfs:label          "unit of effort"@en ;
        rdfs:domain         vf:EconomicResource ;
        rdfs:range          vf:Unit ;
        owl:maxCardinality  1 ;
        vs:term_status      "stable" ;
        rdfs:comment        "The unit used for use or work or sometimes cite actions."@en ;
        .

vf:defaultUnitOfEffort a    owl:ObjectProperty ;
        rdfs:label          "default unit of effort"@en ;
        rdfs:domain         vf:ResourceSpecification ;
        rdfs:range          vf:Unit ;
        owl:maxCardinality  1 ;
        vs:term_status      "testing" ;
        rdfs:comment        "The default unit used for use or work."@en ;
        .

vf:defaultUnitOfResource a  owl:ObjectProperty ;
        rdfs:label          "default unit of resource"@en ;
        rdfs:domain         vf:ResourceSpecification ;
        rdfs:range          vf:Unit ;
        owl:maxCardinality  1 ;
        vs:term_status      "testing" ;
        rdfs:comment        "The default unit used for the resource itself."@en ;
        .

vf:basedOn
        a                   owl:ObjectProperty ;
        rdfs:label          "based on"@en ;
        rdfs:domain         vf:Process ;
        rdfs:range          vf:ProcessSpecification ;
        owl:maxCardinality  1 ;
        vs:term_status      "stable" ;
        rdfs:comment        "The definition or standard specification for a process."@en ;
        .

vf:classifiedAs
        a                   owl:ObjectProperty ;
        rdfs:label          "classified as"@en ;
        rdfs:domain         [ owl:unionOf (vf:Process vf:EconomicResource vf:Organization vf:EcologicalAgent vf:Unit) ] ;
        rdfs:range          xsd:string ;
        vs:term_status      "unstable" ;
        rdfs:comment        "References one or more uri's for a concept in a common taxonomy or other classification scheme for purposes of categorization or grouping; or can be one or more string classifications."@en ;
        .

vf:resourceClassifiedAs
        a                   owl:ObjectProperty ;
        rdfs:label          "resource classified as"@en ;
        rdfs:domain         [ owl:unionOf (vf:ResourceSpecification vf:RecipeFlow vf:Intent vf:Commitment vf:EconomicEvent vf:Claim) ] ;
        rdfs:range          xsd:string ;
        vs:term_status      "unstable" ;
        rdfs:comment        "References one or more uri's for a concept in a common taxonomy or other classification scheme for purposes of categorization or grouping; or can be one or more string classifications."@en ;
        .

vf:processClassifiedAs
        a                   owl:ObjectProperty ;
        rdfs:label          "process classified as"@en ;
        rdfs:domain         vf:RecipeProcess ;
        rdfs:range          xsd:string ;
        vs:term_status      "unstable" ;
        rdfs:comment        "References one or more uri's for a concept in a common taxonomy or other classification scheme for purposes of categorization or grouping; or can be one or more string classifications."@en ;
        .

vf:processConformsTo
        a                   owl:ObjectProperty ;
        rdfs:label          "process conforms to"@en ;
        rdfs:domain         vf:RecipeProcess ;
        rdfs:range          vf:ProcessSpecification ;
        owl:maxCardinality  1 ;
        vs:term_status      "stable" ;
        rdfs:comment        "The standard specification or definition of a process."@en ;
        .

vf:resourceConformsTo
        a                   owl:ObjectProperty ;
        rdfs:label          "resource conforms to"@en ;
        rdfs:domain         [ owl:unionOf (vf:Commitment vf:Intent vf:EconomicEvent vf:Claim vf:RecipeFlow) ] ;
        rdfs:range          vf:ResourceSpecification ;
        owl:maxCardinality  1 ;
        vs:term_status      "stable" ;
        rdfs:comment        "The primary resource specification or definition of an existing or potential economic resource. A resource will have only one, as this specifies exactly what the resource is."@en ;
        .

vf:conformsTo
        a                   owl:ObjectProperty ;
        rdfs:label          "conforms to"@en ;
        rdfs:domain         vf:EconomicResource ;
        rdfs:range          vf:ResourceSpecification ;
        owl:maxCardinality  1 ;
        vs:term_status      "stable" ;
        rdfs:comment        "The primary resource knowledge specification or definition of an existing or potential resource."@en ;
        .

vf:stage
        a                   owl:ObjectProperty ;
        rdfs:label          "stage"@en ;
        rdfs:domain         [ owl:unionOf (vf:EconomicResource vf:Commitment vf:RecipeFlow) ] ;
        rdfs:range          vf:ProcessSpecification ;
        owl:maxCardinality  1 ;
        vs:term_status      "stable" ;
        rdfs:comment        "References the ProcessSpecification of the last process the economic resource went through. Stage is used when the last process is important for finding proper resources, such as where the publishing process wants only documents that have gone through the editing process."@en ;
        .

vf:state
        a                   owl:ObjectProperty ;
        rdfs:label          "state"@en ;
        rdfs:domain         [ owl:unionOf (vf:EconomicResource vf:EconomicEvent vf:RecipeFlow vf:Commitment) ] ;
        rdfs:range          xsd:string ;
        owl:maxCardinality  1 ;
        vs:term_status      "testing" ;
        rdfs:comment        "The state of the desired economic resource, after coming out of a test or review process."@en ;
        .

vf:refinementOf
        a                   owl:ObjectProperty ;
        rdfs:label          "refinement of"@en ;
        rdfs:domain         [ owl:unionOf (vf:Scenario vf:Plan) ] ;
        rdfs:range          vf:Scenario ;
        vs:term_status      "unstable" ;
        rdfs:comment        "This scenario or plan refines another scenario, often as time moves closer or for more detail."@en ;
        .

vf:nestedIn
        a                   owl:ObjectProperty ;
        rdfs:label          "nested in"@en ;
        rdfs:domain         vf:Process ;
        rdfs:range          vf:Scenario ;
        vs:term_status      "unstable" ;
        rdfs:comment        "The process with its inputs and outputs is part of the scenario."@en ;
        .

vf:scenarioIncludes
        a                   owl:ObjectProperty ;
        owl:inverseOf       vf:nestedIn ;
        rdfs:label          "scenario includes"@en ;
        rdfs:domain         vf:Scenario ;
        rdfs:range          [ owl:unionOf (vf:Process vf:Intent) ] ;
        vs:term_status      "testing" ;
        rdfs:comment        "The processes and and/or intents that constitute the plan."@en ;
        .

vf:definedAs
        a                   owl:ObjectProperty ;
        rdfs:label          "defined as"@en ;
        rdfs:domain         vf:Scenario ;
        rdfs:range          vf:ScenarioDefinition ;
        owl:maxCardinality  1 ;
        vs:term_status      "unstable" ;
        rdfs:comment        "The scenario definition for this scenario, for example yearly budget."@en ;
        .

vf:clauseOf a               owl:ObjectProperty ;
        rdfs:label          "clause of"@en ;
        rdfs:domain         vf:Commitment ;
        rdfs:range          vf:Agreement ;
        owl:maxCardinality  1 ;
        vs:term_status      "stable" ;
        rdfs:comment        "This commitment is a primary part of the agreement."@en ;
        .

vf:reciprocalClauseOf a     owl:ObjectProperty ;
        rdfs:label          "reciprocal clause of"@en ;
        rdfs:domain         vf:Commitment ;
        rdfs:range          vf:Agreement ;
        owl:maxCardinality  1 ;
        vs:term_status      "stable" ;
        rdfs:comment        "This commitment is a reciprocal part of the agreement."@en ;
        .

vf:stipulates a             owl:ObjectProperty ;
        owl:inverseOf       vf:clauseOf ;
        rdfs:label          "stipulates"@en ;
        rdfs:domain         vf:Agreement ;
        rdfs:range          vf:Commitment ;
        vs:term_status      "testing" ;
        rdfs:comment        "All the primary commitments that constitute the agreement."@en ;
        .

vf:stipulatesReciprocal a   owl:ObjectProperty ;
        owl:inverseOf       vf:reciprocalClauseOf ;
        rdfs:label          "stipulates reciprocal"@en ;
        rdfs:domain         vf:Agreement ;
        rdfs:range          vf:Commitment ;
        vs:term_status      "testing" ;
        rdfs:comment        "All the reciprocal commitments that constitute the agreement."@en ;
        .

vf:realizationOf a          owl:ObjectProperty ;
        rdfs:label          "realization of"@en ;
        rdfs:domain         vf:EconomicEvent ;
        rdfs:range          vf:Agreement ;
        owl:maxCardinality  1 ;
        vs:term_status      "stable" ;
        rdfs:comment        "This non-reciprocal economic event occurs as part of this agreement."@en ;
        .

vf:realizes a               owl:ObjectProperty ;
        owl:inverseOf       vf:realizationOf ;
        rdfs:label          "realizes"@en ;
        rdfs:domain         vf:Agreement ;
        rdfs:range          vf:EconomicEvent ;
        vs:term_status      "testing" ;
        rdfs:comment        "All the non-reciprocal economic events (with or without commitments) that realize the agreement."@en ;
        .

vf:reciprocalRealizationOf
        a                   owl:ObjectProperty ;
        rdfs:label          "reciprocal realization of"@en ;
        rdfs:domain         vf:EconomicEvent ;
        rdfs:range          vf:Agreement ;
        owl:maxCardinality  1 ;
        vs:term_status      "stable" ;
        rdfs:comment        "This reciprocal economic event occurs as part of this agreement."@en ;
        .

vf:realizesReciprocal a     owl:ObjectProperty ;
        owl:inverseOf       vf:reciprocalRealizationOf ;
        rdfs:label          "realizes reciprocal"@en ;
        rdfs:domain         vf:Agreement ;
        rdfs:range          vf:EconomicEvent ;
        vs:term_status      "testing" ;
        rdfs:comment        "All the reciprocal economic events (with or without commitments) that realize the agreement."@en ;
        .

vf:bundledIn a              owl:ObjectProperty ;
        rdfs:label          "bundled in"@en ;
        rdfs:domain         vf:Agreement ;
        rdfs:range          vf:AgreementBundle ;
        owl:maxCardinality  1 ;
        vs:term_status      "testing" ;
        rdfs:comment        "This agreement is bundled with other agreements."@en ;
        .

vf:bundles a                owl:ObjectProperty ;
        owl:inverseOf       vf:bundledIn ;
        rdfs:label          "bundles"@en ;
        rdfs:domain         vf:AgreementBundle ;
        rdfs:range          vf:Agreement ;
        vs:term_status      "testing" ;
        rdfs:comment        "All the agreements included in this agreement bundle."@en ;
        .

vf:rules a                  owl:DataTypeProperty ;
        rdfs:label          "rules"@en ;
        rdfs:domain         vf:Agreement ;
        rdfs:range          xsd:anyURI ;
        vs:term_status      "unstable" ;
        rdfs:comment        "The rules or contract that govern this agreement."@en ;
        .

vf:roleLabel a              owl:DatatypeProperty ;
        rdfs:label          "role label"@en ;
        rdfs:domain         vf:AgentRelationshipRole ;
        rdfs:range          xsd:string ;
        owl:cardinality     1 ;
        vs:term_status      "stable" ;
        rdfs:comment        "The human readable name of the role, inverse from the object to the subject. For example, 'is member of'."@en ;
        .

vf:inverseRoleLabel a       owl:DatatypeProperty ;
        rdfs:label          "inverse role label"@en ;
        rdfs:domain         vf:AgentRelationshipRole ;
        rdfs:range          xsd:string ;
        owl:maxCardinality  1 ;
        vs:term_status      "stable" ;
        rdfs:comment        "The human readable name of the role, inverse from the object to the subject. For example, 'has member'."@en ;
        .

## Action behaviors

vf:inputOutput a            owl:ObjectProperty ;
        rdfs:domain         vf:Action ;
        rdfs:range          vf:InputOutput ;
        rdfs:comment        "Denotes if a process input or output, or not related to a process."@en ;
        rdfs:label          "input/output"@en ;
        owl:maxCardinality  1 ;
        vs:term_status      "testing" ;
        .

vf:pairsWith a              owl:ObjectProperty ;
        rdfs:domain         vf:Action ;
        rdfs:range          vf:Action ;
        rdfs:comment        "The action that usually affects the same resource as a complement in the same flow."@en ;
        rdfs:label          "pairs with"@en ;
        owl:maxCardinality  1 ;
        vs:term_status      "testing" ;
        .

vf:createResource a         owl:ObjectProperty ;
        rdfs:domain         vf:Action ;
        rdfs:range          vf:CreateResource ;
        rdfs:comment        "The action can create an economic resource."@en ;
        rdfs:label          "can create resource"@en ;
        owl:maxCardinality  1 ;
        vs:term_status      "testing" ;
        .

vf:eventQuantity a          owl:ObjectProperty ;
        rdfs:domain         vf:Action ;
        rdfs:range          vf:EventQuantity ;
        rdfs:comment        "The event quantity applicable is resource quantity, effort quantity, or both."@en ;
        rdfs:label          "event quantity"@en ;
        owl:maxCardinality  1 ;
        vs:term_status      "testing" ;
        .

vf:accountingEffect a       owl:ObjectProperty ;
        rdfs:domain         vf:Action ;
        rdfs:range          vf:AccountingEffect ;
        rdfs:comment        "The increment and/or decrement effect the action will have on the accounting quantity of an inventoried resource."@en ;
        rdfs:label          "accounting effect"@en ;
        owl:maxCardinality  1 ;
        vs:term_status      "testing" ;
        .

vf:onhandEffect a           owl:ObjectProperty ;
        rdfs:domain         vf:Action ;
        rdfs:range          vf:OnhandEffect ;
        rdfs:comment        "The increment and/or decrement effect the action will have on the onhand quantity of an inventoried resource."@en ;
        rdfs:label          "onhand effect"@en ;
        owl:maxCardinality  1 ;
        vs:term_status      "testing" ;
        .

vf:locationEffect a         owl:ObjectProperty ;
        rdfs:domain         vf:Action ;
        rdfs:range          vf:LocationEffect ;
        rdfs:comment        "This action can update the current location of an inventoried resource."@en ;
        rdfs:label          "location effect"@en ;
        owl:maxCardinality  1 ;
        vs:term_status      "testing" ;
        .

vf:containedEffect a        owl:ObjectProperty ;
        rdfs:domain         vf:Action ;
        rdfs:range          vf:ContainedEffect ;
        rdfs:comment        "The contained in resource should be updated or removed."@en ;
        rdfs:label          "contained effect"@en ;
        owl:maxCardinality  1 ;
        vs:term_status      "testing" ;
        .

vf:accountableEffect a      owl:ObjectProperty ;
        rdfs:domain         vf:Action ;
        rdfs:range          vf:AccountableEffect ;
        rdfs:comment        "The primaryAccountable should be updated to the event receiver, or not."@en ;
        rdfs:label          "accountable effect"@en ;
        owl:maxCardinality  1 ;
        vs:term_status      "testing" ;
        .

vf:stageEffect a            owl:ObjectProperty ;
        rdfs:domain         vf:Action ;
        rdfs:range          vf:StageEffect ;
        rdfs:comment        "The stage of the inventoried resource should be updated, or not."@en ;
        rdfs:label          "stage effect"@en ;
        owl:maxCardinality  1 ;
        vs:term_status      "testing" ;
        .
vf:stateEffect a            owl:ObjectProperty ;
        rdfs:domain         vf:Action ;
        rdfs:range          vf:StateEffect ;
        rdfs:comment        "The state of the from or to inventoried resource should be updated, or not."@en ;
        rdfs:label          "state effect"@en ;
        owl:maxCardinality  1 ;
        vs:term_status      "testing" ;
        .

#################################################################
#    Individuals
#################################################################

# Actions

vf:accept a                 owl:NamedIndividual ,
                            vf:Action ;
        vf:inputOutput      vf:input ;
        vf:pairsWith        vf:modify ;
        vf:createResource   vf:notApplicable ;
        vf:eventQuantity    vf:resource ;
        vf:accountingEffect vf:notApplicable ;
        vf:onhandEffect     vf:decrement ;
        vf:locationEffect   vf:update ;
        vf:containedEffect  vf:notApplicable ;
        vf:accountableEffect vf:notApplicable ;
        vf:stageEffect      vf:notApplicable ;
        vf:stateEffect      vf:update ;
        rdfs:comment        "In processes like repair or modification or testing, the same resource will appear in the output."@en ;
        rdfs:label          "accept"@en ;
        vs:term_status      "stable" ;
        .

vf:combine a                owl:NamedIndividual ,
                            vf:Action ;
        vf:inputOutput      vf:input ;
        vf:pairsWith        vf:notApplicable ;
        vf:createResource   vf:notApplicable ;
        vf:eventQuantity    vf:resource ;
        vf:accountingEffect vf:notApplicable ;
        vf:onhandEffect     vf:decrement ;
        vf:locationEffect   vf:notApplicable ;
        vf:containedEffect  vf:update ;
        vf:accountableEffect vf:notApplicable ;
        vf:stageEffect      vf:notApplicable ;
        vf:stateEffect      vf:update ;
        rdfs:comment        "A resource is combined with other resources into a container resource."@en ;
        rdfs:label          "combine"@en ;
        vs:term_status      "unstable" ;
        .

vf:consume a                owl:NamedIndividual ,
                            vf:Action ;
        vf:inputOutput      vf:input ;
        vf:pairsWith        vf:notApplicable ;
        vf:createResource   vf:notApplicable ;
        vf:eventQuantity    vf:resource ;
        vf:accountingEffect vf:decrement ;
        vf:onhandEffect     vf:decrement ;
        vf:locationEffect   vf:notApplicable ;
        vf:containedEffect  vf:notApplicable ;
        vf:accountableEffect vf:notApplicable ;
        vf:stageEffect      vf:notApplicable ;
        vf:stateEffect      vf:update ;
        rdfs:comment        "For example an ingredient or component composed into the output, after the process the ingredient is gone."@en ;
        rdfs:label          "consume"@en ;
        vs:term_status      "stable" ;
        .

vf:cite a                   owl:NamedIndividual ,
                            vf:Action ;
        vf:inputOutput      vf:input ;
        vf:pairsWith        vf:notApplicable ;
        vf:createResource   vf:notApplicable ;
        vf:eventQuantity    vf:resource ;
        vf:accountingEffect vf:notApplicable ;
        vf:onhandEffect     vf:notApplicable ;
        vf:locationEffect   vf:notApplicable ;
        vf:containedEffect  vf:notApplicable ;
        vf:accountableEffect vf:notApplicable ;
        vf:stageEffect      vf:notApplicable ;
        vf:stateEffect      vf:update ;
        rdfs:comment        "For example a design file, neither used nor consumed, the file remains available at all times."@en ;
        rdfs:label          "cite"@en ;
        vs:term_status      "stable" ;
        .

vf:copy a                   owl:NamedIndividual ,
                            vf:Action ;
        vf:inputOutput      vf:notApplicable ;
        vf:pairsWith        vf:notApplicable ;
        vf:createResource   vf:optionalTo ;
        vf:eventQuantity    vf:resource ;
        vf:accountingEffect vf:incrementTo ;
        vf:onhandEffect     vf:incrementTo ;
        vf:locationEffect   vf:new ;
        vf:containedEffect  vf:notApplicable ;
        vf:accountableEffect vf:new ;
        vf:stageEffect      vf:notApplicable ;
        vf:stateEffect      vf:updateTo ;
        rdfs:comment        "Create a new version of the resource, without any change to the original."@en ;
        rdfs:label          "copy"@en ;
        vs:term_status      "unstable" ;
        .

vf:deliverService a         owl:NamedIndividual ,
                            vf:Action ;
        vf:inputOutput      vf:outputInput ;
        vf:pairsWith        vf:notApplicable ;
        vf:createResource   vf:notApplicable ;
        vf:eventQuantity    vf:resource ;
        vf:accountingEffect vf:notApplicable ;
        vf:onhandEffect     vf:notApplicable ;
        vf:locationEffect   vf:notApplicable ;
        vf:containedEffect  vf:notApplicable ;
        vf:accountableEffect vf:notApplicable ;
        vf:stageEffect      vf:notApplicable ;
        vf:stateEffect      vf:notApplicable ;
        rdfs:comment        "New service produced and delivered (a service implies that an agent actively receives the service)."@en ;
        rdfs:label          "deliver service"@en ;
        vs:term_status      "stable" ;
        .

vf:dropoff a                owl:NamedIndividual ,
                            vf:Action ;
        vf:createResource   vf:notApplicable ;
        vf:eventQuantity    vf:resource ;
        vf:inputOutput      vf:output ;
        vf:pairsWith        vf:pickup ;
        vf:accountingEffect vf:notApplicable ;
        vf:onhandEffect     vf:notApplicable ;
        vf:locationEffect   vf:update ;
        vf:containedEffect  vf:notApplicable ;
        vf:accountableEffect vf:notApplicable ;
        vf:stageEffect      vf:update ;
        vf:stateEffect      vf:update ;
        rdfs:comment        "Transported resource or person leaves the process; the same resource or person appeared in the input."@en ;
        rdfs:label          "dropoff"@en ;
        vs:term_status      "stable" ;
        .

vf:lower a                  owl:NamedIndividual ,
                            vf:Action ;
        vf:inputOutput      vf:notApplicable ;
        vf:createResource   vf:optional ;
        vf:eventQuantity    vf:resource ;
        vf:pairsWith        vf:notApplicable ;
        vf:accountingEffect vf:decrement ;
        vf:onhandEffect     vf:decrement ;
        vf:locationEffect   vf:notApplicable ;
        vf:containedEffect  vf:notApplicable ;
        vf:accountableEffect vf:new ;
        vf:stageEffect      vf:notApplicable ;
        vf:stateEffect      vf:update ;
        rdfs:comment        "Adjusts a quantity down based on a beginning balance or inventory count."@en ;
        rdfs:label          "lower"@en ;
        vs:term_status      "stable" ;
        .

vf:modify a                 owl:NamedIndividual ,
                            vf:Action ;
        vf:createResource   vf:notApplicable ;
        vf:eventQuantity    vf:resource ;
        vf:inputOutput      vf:output ;
        vf:pairsWith        vf:accept ;
        vf:accountingEffect vf:notApplicable ;
        vf:onhandEffect     vf:increment ;
        vf:locationEffect   vf:update ;
        vf:containedEffect  vf:notApplicable ;
        vf:accountableEffect vf:notApplicable ;
        vf:stageEffect      vf:update ;
        vf:stateEffect      vf:update ;
        rdfs:comment        "In processes like repair or modification, the same resource will appear in the input."@en ;
        rdfs:label          "modify"@en ;
        vs:term_status      "stable" ;
        .

vf:move a                   owl:NamedIndividual ,
                            vf:Action ;
        vf:inputOutput      vf:notApplicable ;
        vf:pairsWith        vf:notApplicable ;
        vf:createResource   vf:optionalTo ;
        vf:eventQuantity    vf:resource ;
        vf:accountingEffect vf:decrementIncrement ;
        vf:onhandEffect     vf:decrementIncrement ;
        vf:locationEffect   vf:updateTo ;
        vf:containedEffect  vf:notApplicable ;
        vf:accountableEffect vf:notApplicable ;
        vf:stageEffect      vf:notApplicable ;
        vf:stateEffect      vf:updateTo ;
        rdfs:comment        "Change location and possibly identifier, if location is part of the identification, of a resource with no change of agent rights or possession."@en ;
        rdfs:label          "move"@en ;
        vs:term_status      "testing" ;
        .

vf:pickup a                 owl:NamedIndividual ,
                            vf:Action ;
        vf:inputOutput      vf:input ;
        vf:pairsWith        vf:dropoff ;
        vf:createResource   vf:notApplicable ;
        vf:eventQuantity    vf:resource ;
        vf:accountingEffect vf:notApplicable ;
        vf:onhandEffect     vf:notApplicable ;
        vf:locationEffect   vf:update ;
        vf:containedEffect  vf:notApplicable ;
        vf:accountableEffect vf:notApplicable ;
        vf:stageEffect      vf:notApplicable ;
        vf:stateEffect      vf:update ;
        rdfs:comment        "Transported resource or person enters the process; the same resource will appear in the output."@en ;
        rdfs:label          "pickup"@en ;
        vs:term_status      "stable" ;
        .

vf:produce a                owl:NamedIndividual ,
                            vf:Action ;
        vf:inputOutput      vf:output ;
        vf:pairsWith        vf:notApplicable ;
        vf:createResource   vf:optional ;
        vf:eventQuantity    vf:resource ;
        vf:accountingEffect vf:increment ;
        vf:onhandEffect     vf:increment ;
        vf:locationEffect   vf:new ;
        vf:containedEffect  vf:notApplicable ;
        vf:accountableEffect vf:new ;
        vf:stageEffect      vf:update ;
        vf:stateEffect      vf:update ;
        rdfs:comment        "New resource was created in that process or an existing stock resource was added to."@en ;
        rdfs:label          "produce"@en ;
        vs:term_status      "stable" ;
        .

vf:raise a                  owl:NamedIndividual ,
                            vf:Action ;
        vf:inputOutput      vf:notApplicable ;
        vf:pairsWith        vf:notApplicable ;
        vf:createResource   vf:optional ;
        vf:eventQuantity    vf:resource ;
        vf:accountingEffect vf:increment ;
        vf:onhandEffect     vf:increment ;
        vf:locationEffect   vf:notApplicable ;
        vf:containedEffect  vf:notApplicable ;
        vf:accountableEffect vf:new ;
        vf:stageEffect      vf:notApplicable ;
        vf:stateEffect      vf:update ;
        rdfs:comment        "Adjusts a quantity up based on a beginning balance or inventory count."@en ;
        rdfs:label          "raise"@en ;
        vs:term_status      "stable" ;
        .

vf:separate a               owl:NamedIndividual ,
                            vf:Action ;
        vf:inputOutput      vf:output ;
        vf:pairsWith        vf:notApplicable ;
        vf:createResource   vf:notApplicable ;
        vf:eventQuantity    vf:resource ;
        vf:accountingEffect vf:notApplicable ;
        vf:onhandEffect     vf:increment ;
        vf:locationEffect   vf:notApplicable ;
        vf:containedEffect  vf:remove ;
        vf:accountableEffect vf:notApplicable ;
        vf:stageEffect      vf:update ;
        vf:stateEffect      vf:update ;
        rdfs:comment        "A resource is removed from a container resource."@en ;
        rdfs:label          "unpack"@en ;
        vs:term_status      "testing" ;
        .

vf:transferAllRights a      owl:NamedIndividual ,
                            vf:Action ;
        vf:inputOutput      vf:notApplicable ;
        vf:pairsWith        vf:notApplicable ;
        vf:createResource   vf:optionalTo ;
        vf:eventQuantity    vf:resource ;
        vf:accountingEffect vf:decrementIncrement ;
        vf:onhandEffect     vf:notApplicable ;
        vf:locationEffect   vf:notApplicable ;
        vf:containedEffect  vf:notApplicable ;
        vf:accountableEffect vf:updateTo ;
        vf:stageEffect      vf:notApplicable ;
        vf:stateEffect      vf:updateTo ;
        rdfs:comment        "Give full (in the human realm) rights and responsibilities to another agent, without transferring physical custody."@en ;
        rdfs:label          "transfer all rights"@en ;
        vs:term_status      "testing" ;
        .

vf:transfer a               owl:NamedIndividual ,
                            vf:Action ;
        vf:inputOutput      vf:notApplicable ;
        vf:pairsWith        vf:notApplicable ;
        vf:createResource   vf:optionalTo ;
        vf:eventQuantity    vf:resource ;
        vf:accountingEffect vf:decrementIncrement ;
        vf:onhandEffect     vf:decrementIncrement ;
        vf:locationEffect   vf:updateTo ;
        vf:containedEffect  vf:notApplicable ;
        vf:accountableEffect vf:updateTo ;
        vf:stageEffect      vf:notApplicable ;
        vf:stateEffect      vf:updateTo ;
        rdfs:comment        "Give full rights and responsibilities plus physical custody."@en ;
        rdfs:label          "transfer"@en ;
        vs:term_status      "stable" ;
        .

vf:transferCustody a        owl:NamedIndividual ,
                            vf:Action ;
        vf:inputOutput      vf:notApplicable ;
        vf:pairsWith        vf:notApplicable ;
        vf:createResource   vf:optionalTo ;
        vf:eventQuantity    vf:resource ;
        vf:accountingEffect vf:notApplicable ;
        vf:onhandEffect     vf:decrementIncrement ;
        vf:locationEffect   vf:updateTo ;
        vf:containedEffect  vf:notApplicable ;
        vf:accountableEffect vf:notApplicable ;
        vf:stageEffect      vf:notApplicable ;
        vf:stateEffect      vf:updateTo ;
        rdfs:comment        "Give physical custody and control of a resource, without full accounting or ownership rights."@en ;
        rdfs:label          "transfer custody"@en ;
        vs:term_status      "testing" ;
        .

vf:use a                    owl:NamedIndividual ,
                            vf:Action ;
        vf:inputOutput      vf:input ;
        vf:pairsWith        vf:notApplicable ;
        vf:createResource   vf:notApplicable ;
        vf:eventQuantity    vf:both ;
        vf:accountingEffect vf:notApplicable ;
        vf:onhandEffect     vf:notApplicable ;
        vf:locationEffect   vf:notApplicable ;
        vf:containedEffect  vf:notApplicable ;
        vf:accountableEffect vf:notApplicable ;
        vf:stageEffect      vf:notApplicable ;
        vf:stateEffect      vf:update ;
        rdfs:comment        "For example a tool used in process; after the process, the tool still exists."@en ;
        rdfs:label          "use"@en ;
        vs:term_status      "stable" ;
        .

vf:work a                   owl:NamedIndividual ,
                            vf:Action ;
        vf:inputOutput      vf:input ;
        vf:pairsWith        vf:notApplicable ;
        vf:createResource   vf:notApplicable ;
        vf:eventQuantity    vf:effort ;
        vf:accountingEffect vf:notApplicable ;
        vf:onhandEffect     vf:notApplicable ;
        vf:locationEffect   vf:notApplicable ;
        vf:containedEffect  vf:notApplicable ;
        vf:accountableEffect vf:notApplicable ;
        vf:stageEffect      vf:notApplicable ;
        vf:stateEffect      vf:notApplicable ;
        rdfs:comment        "Labor power applied to a process."@en ;
        rdfs:label          "work"@en ;
        vs:term_status      "stable" ;
        .

# Resource effects

vf:decrement a              owl:NamedIndividual ,
                            vf:AccountingEffect ,
                            vf:OnhandEffect ;
        rdfs:comment        "The effect is to subtract from the inventoried resource accounting or onhand quantity."@en ;
        rdfs:label          "decrement"@en ;
        vs:term_status      "stable" ;
        .

vf:decrementIncrement a     owl:NamedIndividual ,
                            vf:AccountingEffect ,
                            vf:OnhandEffect ;
        rdfs:comment        "The effect is to subtract from the 'from' inventoried resource, and add to the 'to' inventoried resource, accounting or onhand quantity."@en ;
        rdfs:label          "decrement/increment"@en ;
        vs:term_status      "stable" ;
        .

vf:increment a              owl:NamedIndividual ,
                            vf:AccountingEffect ,
                            vf:OnhandEffect ;
        rdfs:comment        "The effect is to add to the inventoried resource accounting or onhand quantity."@en ;
        rdfs:label          "increment"@en ;
        vs:term_status      "stable" ;
        .

vf:incrementTo a            owl:NamedIndividual ,
                            vf:AccountingEffect ,
                            vf:OnhandEffect ;
        rdfs:comment        "The effect is to add to the to (receiver) inventoried resource accounting or onhand quantity."@en ;
        rdfs:label          "increment to"@en ;
        vs:term_status      "stable" ;
        .

vf:update a                 owl:NamedIndividual ,
                            vf:ContainedEffect ,
                            vf:StageEffect ,
                            vf:StateEffect ,
                            vf:LocationEffect ;
        rdfs:comment        "The effect is to update the resource in the specified property."@en ;
        rdfs:label          "update"@en ;
        vs:term_status      "testing" ;
        .

vf:updateTo a               owl:NamedIndividual ,
                            vf:ContainedEffect ,
                            vf:StateEffect ,
                            vf:AccountableEffect ,
                            vf:LocationEffect ;
        rdfs:comment        "The effect is to update the to resource in the specified property."@en ;
        rdfs:label          "update"@en ;
        vs:term_status      "testing" ;
        .

vf:remove a                 owl:NamedIndividual ,
                            vf:ContainedEffect ;
        rdfs:comment        "The effect is to remove or nullify the specified property from the resource."@en ;
        rdfs:label          "remove"@en ;
        vs:term_status      "testing" ;
        .

vf:new a                    owl:NamedIndividual ,
                            vf:AccountableEffect ,
                            vf:LocationEffect ;
        rdfs:comment        "The effect applies for a new resource created by the event."@en ;
        rdfs:label          "remove"@en ;
        vs:term_status      "testing" ;
        .

# Input/output

vf:input a                  owl:NamedIndividual ,
                            vf:InputOutput ;
        rdfs:comment        "This kind of flow can be an input to a process."@en ;
        rdfs:label          "input"@en ;
        vs:term_status      "stable" ;
        .

vf:output a                 owl:NamedIndividual ,
                            vf:InputOutput ;
        rdfs:comment        "This kind of flow can be an output to a process."@en ;
        rdfs:label          "output"@en ;
        vs:term_status      "stable" ;
        .

vf:outputInput a            owl:NamedIndividual ,
                            vf:InputOutput ;
        rdfs:comment        "This kind of flow can be an output to a process, and at the same time an input to another process."@en ;
        rdfs:label          "output input"@en ;
        vs:term_status      "testing" ;
        .

# Event behavior

vf:resource  a              owl:NamedIndividual ,
                            vf:EventQuantity ;
        rdfs:comment        "This event uses resourceQuantity."@en ;
        rdfs:label          "resource"@en ;
        vs:term_status      "testing" ;
        .

vf:effort  a                owl:NamedIndividual ,
                            vf:EventQuantity ;
        rdfs:comment        "This event uses effortQuantity."@en ;
        rdfs:label          "effort"@en ;
        vs:term_status      "testing" ;
        .

vf:both  a                  owl:NamedIndividual ,
                            vf:EventQuantity ;
        rdfs:comment        "This event can use resourceQuantity and effortQuantity."@en ;
        rdfs:label          "both"@en ;
        vs:term_status      "testing" ;
        .

# Create a new resource behavior
        
vf:optional  a              owl:NamedIndividual ,
                            vf:CreateResource ;
        rdfs:comment        "This kind of flow gives the user the option to create a new resource using resourceInventoriedAs."@en ;
        rdfs:label          "optional"@en ;
        vs:term_status      "testing" ;
        .

vf:optionalTo  a            owl:NamedIndividual ,
                            vf:CreateResource ;
        rdfs:comment        "This kind of flow gives the user the option to create a new resource using toResourceInventoriedAs."@en ;
        rdfs:label          "optional to"@en ;
        vs:term_status      "testing" ;
        .

# Not applicable

vf:notApplicable a          owl:NamedIndividual ,
                            vf:InputOutput ,
                            vf:PairsWith ,
                            vf:LocationEffect ,
                            vf:CreateResource ,
                            vf:ContainedEffect;
        rdfs:comment        "This property is not applicable to this kind of flow."@en ;
        rdfs:label          "not applicable"@en ;
        vs:term_status      "testing" ;
        .

# Proposal Purpose choices

vf:offer a                  owl:NamedIndividual ,
                            vf:ProposalPurpose ;
        rdfs:comment        "The proposal is an offer."@en ;
        rdfs:label          "offer"@en ;
        vs:term_status      "testing" ;
        .

vf:request a                owl:NamedIndividual ,
                            vf:ProposalPurpose ;
        rdfs:comment        "The proposal is a published request, need, want."@en ;
        rdfs:label          "request"@en ;
        vs:term_status      "testing" ;
        .
