{
  "@context": {
    "@base": "https://w3id.org/valueflows/ont/vf",
    "vf": "https://w3id.org/valueflows/ont/vf#",
    "rdf": "http://www.w3.org/1999/02/22-rdf-syntax-ns#",
    "owl": "http://www.w3.org/2002/07/owl#",
    "rdfs": "http://www.w3.org/2000/01/rdf-schema#",
    "dcterms": "http://purl.org/dc/terms/",
    "om2": "http://www.ontology-of-units-of-measure.org/resource/om-2/",
    "xsd": "http://www.w3.org/2001/XMLSchema#",
    "time": "http://www.w3.org/2006/time#",
    "geo": "http://www.w3.org/2003/01/geo/wgs84_pos#",
    "vs": "http://www.w3.org/2003/06/sw-vocab-status/ns#",
    "dtype": "http://www.linkedmodel.org/schema/dtype#",
    "skos": "http://www.w3.org/2004/02/skos/core#"
  },
  "@graph": [
    {
      "@id": "https://w3id.org/valueflows/ont/vf",
      "@type": "owl:Ontology",
      "dcterms:title": "Valueflows Ontology",
      "dcterms:type": {
        "@id": "http://purl.org/adms/assettype/Ontology"
      },
      "owl:versionIRI": {
        "@id": "https://w3id.org/valueflows/ont/0.11/vf"
      },
      "dcterms:status": {
        "@id": "http://purl.org/adms/status/UnderDevelopment"
      }
    },
    {
      "@id": "vf:ResourceSpecification",
      "@type": "owl:Class",
      "rdfs:label": {
        "@value": "Resource Specification",
        "@language": "en"
      },
      "vs:term_status": "stable",
      "rdfs:comment": {
        "@value": "Specifies the kind of resource, even if the resource is not instantiated as an EconomicResource. Could define a material item, service, digital item, currency account, skill or type of work, etc.",
        "@language": "en"
      }
    },
    {
      "@id": "vf:ProcessSpecification",
      "@type": "owl:Class",
      "rdfs:label": {
        "@value": "Process Specification",
        "@language": "en"
      },
      "vs:term_status": "testing",
      "rdfs:comment": {
        "@value": "Specifies the kind of process.",
        "@language": "en"
      }
    },
    {
      "@id": "vf:Action",
      "@type": "owl:Class",
      "rdfs:label": {
        "@value": "Action",
        "@language": "en"
      },
      "vs:term_status": "stable",
      "rdfs:comment": {
        "@value": "An action verb defining the kind of flow and its behavior.",
        "@language": "en"
      }
    },
    {
      "@id": "vf:InputOutput",
      "@type": "owl:Class",
      "rdfs:label": {
        "@value": "Input/Output",
        "@language": "en"
      },
      "vs:term_status": "testing",
      "rdfs:comment": {
        "@value": "The action is an input or output of a process, or not related to a process.",
        "@language": "en"
      }
    },
    {
      "@id": "vf:CreateResource",
      "@type": "owl:Class",
      "rdfs:label": {
        "@value": "Create Resource",
        "@language": "en"
      },
      "vs:term_status": "testing",
      "rdfs:comment": {
        "@value": "The action can create an economic resource.",
        "@language": "en"
      }
    },
    {
      "@id": "vf:EventQuantity",
      "@type": "owl:Class",
      "rdfs:label": {
        "@value": "Event Quantity",
        "@language": "en"
      },
      "vs:term_status": "testing",
      "rdfs:comment": {
        "@value": "The action involves the event resource quantity, event quantity, or both.",
        "@language": "en"
      }
    },
    {
      "@id": "vf:AccountingEffect",
      "@type": "owl:Class",
      "rdfs:label": {
        "@value": "Accounting Effect",
        "@language": "en"
      },
      "vs:term_status": "testing",
      "rdfs:comment": {
        "@value": "The action has this effect on an inventoried resource accounting quantity.",
        "@language": "en"
      }
    },
    {
      "@id": "vf:OnhandEffect",
      "@type": "owl:Class",
      "rdfs:label": {
        "@value": "Onhand Effect",
        "@language": "en"
      },
      "vs:term_status": "testing",
      "rdfs:comment": {
        "@value": "The action has this effect on an inventoried resource onhand quantity.",
        "@language": "en"
      }
    },
    {
      "@id": "vf:LocationEffect",
      "@type": "owl:Class",
      "rdfs:label": {
        "@value": "Location Effect",
        "@language": "en"
      },
      "vs:term_status": "testing",
      "rdfs:comment": {
        "@value": "The action has this effect on an inventoried resource current location.",
        "@language": "en"
      }
    },
    {
      "@id": "vf:ContainedEffect",
      "@type": "owl:Class",
      "rdfs:label": {
        "@value": "Contained Effect",
        "@language": "en"
      },
      "vs:term_status": "testing",
      "rdfs:comment": {
        "@value": "The action has this effect on an inventoried resource contained in resource.",
        "@language": "en"
      }
    },
    {
      "@id": "vf:AccountableEffect",
      "@type": "owl:Class",
      "rdfs:label": {
        "@value": "Accountable Effect",
        "@language": "en"
      },
      "vs:term_status": "testing",
      "rdfs:comment": {
        "@value": "The action has this effect on an inventoried resource primary accountable agent.",
        "@language": "en"
      }
    },
    {
      "@id": "vf:StageEffect",
      "@type": "owl:Class",
      "rdfs:label": {
        "@value": "Stage Effect",
        "@language": "en"
      },
      "vs:term_status": "testing",
      "rdfs:comment": {
        "@value": "The action has this effect on an inventoried resource stage.",
        "@language": "en"
      }
    },
    {
      "@id": "vf:StateEffect",
      "@type": "owl:Class",
      "rdfs:label": {
        "@value": "State Effect",
        "@language": "en"
      },
      "vs:term_status": "unstable",
      "rdfs:comment": {
        "@value": "The action has this effect on an inventoried resource state.",
        "@language": "en"
      }
    },
    {
      "@id": "vf:AgentRelationshipRole",
      "@type": "owl:Class",
      "rdfs:label": {
        "@value": "Agent Relationship Role",
        "@language": "en"
      },
      "vs:term_status": "stable",
      "rdfs:comment": {
        "@value": "A relationship role defining the kind of association one agent can have with another.",
        "@language": "en"
      }
    },
    {
      "@id": "vf:RoleBehavior",
      "@type": "owl:Class",
      "rdfs:label": {
        "@value": "Role Behavior",
        "@language": "en"
      },
      "vs:term_status": "testing",
      "rdfs:comment": {
        "@value": "The general shape or behavior grouping of an agent relationship role.",
        "@language": "en"
      }
    },
    {
      "@id": "vf:Recipe",
      "@type": "owl:Class",
      "rdfs:label": {
        "@value": "Recipe",
        "@language": "en"
      },
      "vs:term_status": "unstable",
      "rdfs:comment": {
        "@value": "Optional instance of a recipe which directly specifies the recipe processes included.",
        "@language": "en"
      }
    },
    {
      "@id": "vf:RecipeGroup",
      "@type": "owl:Class",
      "rdfs:label": {
        "@value": "Recipe Group",
        "@language": "en"
      },
      "vs:term_status": "unstable",
      "rdfs:comment": {
        "@value": "A grouping of recipes to facilitate planning them together.",
        "@language": "en"
      }
    },
    {
      "@id": "vf:RecipeProcess",
      "@type": "owl:Class",
      "rdfs:label": {
        "@value": "Recipe Process",
        "@language": "en"
      },
      "vs:term_status": "stable",
      "rdfs:comment": {
        "@value": "Specifies a process in a recipe for use in planning from recipe.",
        "@language": "en"
      }
    },
    {
      "@id": "vf:RecipeFlow",
      "@type": "owl:Class",
      "rdfs:label": {
        "@value": "Recipe Flow",
        "@language": "en"
      },
      "vs:term_status": "stable",
      "rdfs:comment": {
        "@value": "The specification of a resource inflow to, or outflow from, a recipe process.",
        "@language": "en"
      }
    },
    {
      "@id": "vf:RecipeExchange",
      "@type": "owl:Class",
      "rdfs:label": {
        "@value": "Recipe Exchange",
        "@language": "en"
      },
      "vs:term_status": "testing",
      "rdfs:comment": {
        "@value": "Specifies an exchange type agreement as part of a recipe.",
        "@language": "en"
      }
    },
    {
      "@id": "vf:ScenarioDefinition",
      "@type": "owl:Class",
      "rdfs:label": {
        "@value": "Scenario Definition",
        "@language": "en"
      },
      "vs:term_status": "unstable",
      "rdfs:comment": {
        "@value": "The type definition of one or more scenarios.",
        "@language": "en"
      }
    },
    {
      "@id": "vf:Plan",
      "@type": "owl:Class",
      "rdfs:label": {
        "@value": "Plan",
        "@language": "en"
      },
      "vs:term_status": "stable",
      "rdfs:comment": {
        "@value": "A logical collection of processes that constitute a body of scheduled work with defined deliverable(s).",
        "@language": "en"
      }
    },
    {
      "@id": "vf:Intent",
      "@type": "owl:Class",
      "rdfs:label": {
        "@value": "Intent",
        "@language": "en"
      },
      "vs:term_status": "stable",
      "rdfs:comment": {
        "@value": "A proposed or planned or estimated economic flow, prior to a commitment or agreement, which can lead to commitments and/or economic events.",
        "@language": "en"
      }
    },
    {
      "@id": "vf:Proposal",
      "@type": "owl:Class",
      "rdfs:label": {
        "@value": "Proposal",
        "@language": "en"
      },
      "vs:term_status": "testing",
      "rdfs:comment": {
        "@value": "Published requests or offers, sometimes with what is expected in return.",
        "@language": "en"
      }
    },
    {
      "@id": "vf:ProposalList",
      "@type": "owl:Class",
      "rdfs:label": {
        "@value": "Proposal List",
        "@language": "en"
      },
      "vs:term_status": "unstable",
      "rdfs:comment": {
        "@value": "A grouping of proposals, for publishing as a list.",
        "@language": "en"
      }
    },
    {
      "@id": "vf:ProposalPurpose",
      "@type": "owl:Class",
      "rdfs:label": {
        "@value": "Proposal Purpose",
        "@language": "en"
      },
      "vs:term_status": "testing",
      "rdfs:comment": {
        "@value": "The type of proposal, an offer or request (others may be added).",
        "@language": "en"
      }
    },
    {
      "@id": "vf:Commitment",
      "@type": "owl:Class",
      "rdfs:label": {
        "@value": "Commitment",
        "@language": "en"
      },
      "vs:term_status": "stable",
      "rdfs:comment": {
        "@value": "A planned economic flow that has been promised by an agent to another agent.",
        "@language": "en"
      }
    },
    {
      "@id": "vf:Agreement",
      "@type": "owl:Class",
      "rdfs:label": {
        "@value": "Agreement",
        "@language": "en"
      },
      "vs:term_status": "testing",
      "rdfs:comment": {
        "@value": "Any type of agreement among economic agents.",
        "@language": "en"
      }
    },
    {
      "@id": "vf:AgreementBundle",
      "@type": "owl:Class",
      "rdfs:label": {
        "@value": "Agreement Bundle",
        "@language": "en"
      },
      "vs:term_status": "unstable",
      "rdfs:comment": {
        "@value": "A grouping of agreements to bundle detailed line item reciprocity.",
        "@language": "en"
      }
    },
    {
      "@id": "vf:Scenario",
      "@type": "owl:Class",
      "rdfs:label": {
        "@value": "Scenario",
        "@language": "en"
      },
      "vs:term_status": "unstable",
      "rdfs:comment": {
        "@value": "An estimated or analytical logical collection of higher level processes used for budgeting, analysis, plan refinement, etc.",
        "@language": "en"
      }
    },
    {
      "@id": "vf:Agent",
      "@type": "owl:Class",
      "rdfs:label": {
        "@value": "Agent",
        "@language": "en"
      },
      "vs:term_status": "stable",
      "rdfs:comment": {
        "@value": "An entity that can commit to and/or perform economic and/or ecological activity under its own power or authority.",
        "@language": "en"
      }
    },
    {
      "@id": "vf:Person",
      "@type": "owl:Class",
      "rdfs:label": {
        "@value": "Person",
        "@language": "en"
      },
      "rdfs:subClassOf": {
        "@id": "vf:Agent"
      },
      "vs:term_status": "stable",
      "rdfs:comment": {
        "@value": "A human being. All people are considered agents.",
        "@language": "en"
      }
    },
    {
      "@id": "vf:Organization",
      "@type": "owl:Class",
      "rdfs:label": {
        "@value": "Organization",
        "@language": "en"
      },
      "rdfs:subClassOf": {
        "@id": "vf:Agent"
      },
      "vs:term_status": "stable",
      "rdfs:comment": {
        "@value": "A functional structure, formal or informal, which can include people and/or other organizations, and has its own agency.  Something called a group is an Organization in Valueflows if it has its own agency.",
        "@language": "en"
      }
    },
    {
      "@id": "vf:EcologicalAgent",
      "@type": "owl:Class",
      "rdfs:label": {
        "@value": "Ecological Agent",
        "@language": "en"
      },
      "rdfs:subClassOf": {
        "@id": "vf:Agent"
      },
      "vs:term_status": "testing",
      "rdfs:comment": {
        "@value": "A non-human being; or a functional group of non-human beings; or an ecosystem of living beings that includes non-humans.",
        "@language": "en"
      }
    },
    {
      "@id": "vf:EconomicResource",
      "@type": "owl:Class",
      "rdfs:label": {
        "@value": "Economic Resource",
        "@language": "en"
      },
      "vs:term_status": "stable",
      "rdfs:comment": {
        "@value": "Economic or environmental inputs to or outputs from processes.",
        "@language": "en"
      }
    },
    {
      "@id": "vf:Process",
      "@type": "owl:Class",
      "rdfs:label": {
        "@value": "Process",
        "@language": "en"
      },
      "vs:term_status": "stable",
      "rdfs:comment": {
        "@value": "An activity that changes inputs into outputs, by transforming or transporting economic resource(s).",
        "@language": "en"
      }
    },
    {
      "@id": "vf:EconomicEvent",
      "@type": "owl:Class",
      "rdfs:label": {
        "@value": "Economic Event",
        "@language": "en"
      },
      "vs:term_status": "stable",
      "rdfs:comment": {
        "@value": "An observed economic flow, as opposed to a flow planned to happen in the future. This could reflect a change in the quantity of an economic resource. It is also defined by its behavior in relation to the economic resource (see vf:action)",
        "@language": "en"
      }
    },
    {
      "@id": "vf:AgentRelationship",
      "@type": "owl:Class",
      "rdfs:label": {
        "@value": "Agent Relationship",
        "@language": "en"
      },
      "vs:term_status": "stable",
      "rdfs:comment": {
        "@value": "An ongoing voluntary association between 2 agents of any kind.",
        "@language": "en"
      }
    },
    {
      "@id": "vf:Claim",
      "@type": "owl:Class",
      "rdfs:label": {
        "@value": "Claim",
        "@language": "en"
      },
      "vs:term_status": "unstable",
      "rdfs:comment": {
        "@value": "A claim for a future economic event(s) in reciprocity for an economic event that already occurred. For example, a claim for payment for goods received.",
        "@language": "en"
      }
    },
    {
      "@id": "vf:Appreciation",
      "@type": "owl:Class",
      "rdfs:label": {
        "@value": "Appreciation",
        "@language": "en"
      },
      "vs:term_status": "unstable",
      "rdfs:comment": {
        "@value": "A way to tie an economic event that is given in loose fulfilment for another economic event, without commitments or expectations. Supports the gift economy.",
        "@language": "en"
      }
    },
    {
      "@id": "vf:action",
      "@type": "owl:ObjectProperty",
      "rdfs:label": {
        "@value": "action",
        "@language": "en"
      },
      "rdfs:domain": {
        "owl:unionOf": {
          "@list": [
            {
              "@id": "vf:EconomicEvent"
            },
            {
              "@id": "vf:Commitment"
            },
            {
              "@id": "vf:Intent"
            },
            {
              "@id": "vf:RecipeFlow"
            },
            {
              "@id": "vf:Claim"
            }
          ]
        }
      },
      "rdfs:range": {
        "@id": "vf:Action"
      },
      "vs:term_status": "stable",
      "rdfs:comment": {
        "@value": "Defines the kind of flow, such as consume, produce, work, transfer, etc.",
        "@language": "en"
      }
    },
    {
      "@id": "vf:inputOf",
      "@type": "owl:ObjectProperty",
      "rdfs:label": {
        "@value": "input of",
        "@language": "en"
      },
      "rdfs:domain": {
        "owl:unionOf": {
          "@list": [
            {
              "@id": "vf:EconomicEvent"
            },
            {
              "@id": "vf:Commitment"
            },
            {
              "@id": "vf:Intent"
            }
          ]
        }
      },
      "rdfs:range": {
        "@id": "vf:Process"
      },
      "vs:term_status": "stable",
      "rdfs:comment": {
        "@value": "Relates an input flow to its process.",
        "@language": "en"
      }
    },
    {
      "@id": "vf:hasInput",
      "@type": "owl:ObjectProperty",
      "owl:inverseOf": {
        "@id": "vf:inputOf"
      },
      "rdfs:label": {
        "@value": "has input",
        "@language": "en"
      },
      "rdfs:domain": {
        "@id": "vf:Process"
      },
      "rdfs:range": {
        "owl:unionOf": {
          "@list": [
            {
              "@id": "vf:EconomicEvent"
            },
            {
              "@id": "vf:Commitment"
            },
            {
              "@id": "vf:Intent"
            }
          ]
        }
      },
      "vs:term_status": "testing",
      "rdfs:comment": {
        "@value": "All the input flows of a process.",
        "@language": "en"
      }
    },
    {
      "@id": "vf:outputOf",
      "@type": "owl:ObjectProperty",
      "rdfs:label": {
        "@value": "output of",
        "@language": "en"
      },
      "rdfs:domain": {
        "owl:unionOf": {
          "@list": [
            {
              "@id": "vf:EconomicEvent"
            },
            {
              "@id": "vf:Commitment"
            },
            {
              "@id": "vf:Intent"
            }
          ]
        }
      },
      "rdfs:range": {
        "@id": "vf:Process"
      },
      "vs:term_status": "stable",
      "rdfs:comment": {
        "@value": "Relates an output flow to its process.",
        "@language": "en"
      }
    },
    {
      "@id": "vf:hasOutput",
      "@type": "owl:ObjectProperty",
      "owl:inverseOf": {
        "@id": "vf:outputOf"
      },
      "rdfs:label": {
        "@value": "has output",
        "@language": "en"
      },
      "rdfs:domain": {
        "@id": "vf:Process"
      },
      "rdfs:range": {
        "owl:unionOf": {
          "@list": [
            {
              "@id": "vf:EconomicEvent"
            },
            {
              "@id": "vf:Commitment"
            },
            {
              "@id": "vf:Intent"
            }
          ]
        }
      },
      "vs:term_status": "testing",
      "rdfs:comment": {
        "@value": "All the output flows of a process.",
        "@language": "en"
      }
    },
    {
      "@id": "vf:recipeInputOf",
      "@type": "owl:ObjectProperty",
      "rdfs:label": {
        "@value": "recipe input of",
        "@language": "en"
      },
      "rdfs:domain": {
        "@id": "vf:RecipeFlow"
      },
      "rdfs:range": {
        "@id": "vf:RecipeProcess"
      },
      "vs:term_status": "stable",
      "rdfs:comment": {
        "@value": "Relates an input flow to its process in a recipe.",
        "@language": "en"
      }
    },
    {
      "@id": "vf:hasRecipeInput",
      "@type": "owl:ObjectProperty",
      "owl:inverseOf": {
        "@id": "vf:recipeInputOf"
      },
      "rdfs:label": {
        "@value": "has recipe input",
        "@language": "en"
      },
      "rdfs:domain": {
        "@id": "vf:RecipeProcess"
      },
      "rdfs:range": {
        "@id": "vf:RecipeFlow"
      },
      "vs:term_status": "testing",
      "rdfs:comment": {
        "@value": "All the inputs of a recipe process.",
        "@language": "en"
      }
    },
    {
      "@id": "vf:recipeOutputOf",
      "@type": "owl:ObjectProperty",
      "rdfs:label": {
        "@value": "recipe output of",
        "@language": "en"
      },
      "rdfs:domain": {
        "@id": "vf:RecipeFlow"
      },
      "rdfs:range": {
        "@id": "vf:RecipeProcess"
      },
      "vs:term_status": "stable",
      "rdfs:comment": {
        "@value": "Relates an output flow to its process in a recipe.",
        "@language": "en"
      }
    },
    {
      "@id": "vf:hasRecipeOutput",
      "@type": "owl:ObjectProperty",
      "owl:inverseOf": {
        "@id": "vf:recipeOutputOf"
      },
      "rdfs:label": {
        "@value": "has recipe output",
        "@language": "en"
      },
      "rdfs:domain": {
        "@id": "vf:RecipeProcess"
      },
      "rdfs:range": {
        "@id": "vf:RecipeFlow"
      },
      "vs:term_status": "testing",
      "rdfs:comment": {
        "@value": "All the outputs of a recipe process.",
        "@language": "en"
      }
    },
    {
      "@id": "vf:recipeClauseOf",
      "@type": "owl:ObjectProperty",
      "rdfs:label": {
        "@value": "recipe clause of",
        "@language": "en"
      },
      "rdfs:domain": {
        "@id": "vf:RecipeFlow"
      },
      "rdfs:range": {
        "@id": "vf:RecipeExchange"
      },
      "vs:term_status": "testing",
      "rdfs:comment": {
        "@value": "Relates a flow to its exchange agreement in a recipe.",
        "@language": "en"
      }
    },
    {
      "@id": "vf:recipeStipulates",
      "@type": "owl:ObjectProperty",
      "owl:inverseOf": {
        "@id": "vf:recipeClauseOf"
      },
      "rdfs:label": {
        "@value": "recipe stipulates",
        "@language": "en"
      },
      "rdfs:domain": {
        "@id": "vf:RecipeExchange"
      },
      "rdfs:range": {
        "@id": "vf:RecipeFlow"
      },
      "vs:term_status": "testing",
      "rdfs:comment": {
        "@value": "All the primary clauses of a recipe exchange.",
        "@language": "en"
      }
    },
    {
      "@id": "vf:recipeReciprocalClauseOf",
      "@type": "owl:ObjectProperty",
      "rdfs:label": {
        "@value": "recipe reciprocal clause of",
        "@language": "en"
      },
      "rdfs:domain": {
        "@id": "vf:RecipeFlow"
      },
      "rdfs:range": {
        "@id": "vf:RecipeExchange"
      },
      "vs:term_status": "unstable",
      "rdfs:comment": {
        "@value": "Relates a reciprocal flow to its exchange agreement in a recipe.",
        "@language": "en"
      }
    },
    {
      "@id": "vf:recipeStipulatesReciprocal",
      "@type": "owl:ObjectProperty",
      "owl:inverseOf": {
        "@id": "vf:recipeReciprocalClauseOf"
      },
      "rdfs:label": {
        "@value": "recipe stipulates reciprocal",
        "@language": "en"
      },
      "rdfs:domain": {
        "@id": "vf:RecipeExchange"
      },
      "rdfs:range": {
        "@id": "vf:RecipeFlow"
      },
      "vs:term_status": "unstable",
      "rdfs:comment": {
        "@value": "All the reciprocal clauses of a recipe exchange.",
        "@language": "en"
      }
    },
    {
      "@id": "vf:plannedTogether",
      "@type": "owl:ObjectProperty",
      "rdfs:label": {
        "@value": "planned together",
        "@language": "en"
      },
      "rdfs:domain": {
        "@id": "vf:RecipeGroup"
      },
      "rdfs:range": {
        "@id": "vf:Recipe"
      },
      "vs:term_status": "unstable",
      "rdfs:comment": {
        "@value": "A collection of recipes that can be planned together.",
        "@language": "en"
      }
    },
    {
      "@id": "vf:primaryOutput",
      "@type": "owl:ObjectProperty",
      "rdfs:label": {
        "@value": "primary output",
        "@language": "en"
      },
      "rdfs:domain": {
        "@id": "vf:Recipe"
      },
      "rdfs:range": {
        "@id": "vf:ResourceSpecification"
      },
      "vs:term_status": "unstable",
      "rdfs:comment": {
        "@value": "The main output the recipe is intended to produce or deliver.",
        "@language": "en"
      }
    },
    {
      "@id": "vf:recipeIncludes",
      "@type": "owl:ObjectProperty",
      "rdfs:label": {
        "@value": "recipe includes",
        "@language": "en"
      },
      "rdfs:domain": {
        "@id": "vf:Recipe"
      },
      "rdfs:range": {
        "@id": "vf:RecipeProcess"
      },
      "vs:term_status": "unstable",
      "rdfs:comment": {
        "@value": "The collection of processes needed for this recipe.",
        "@language": "en"
      }
    },
    {
      "@id": "vf:plannedWithin",
      "@type": "owl:ObjectProperty",
      "rdfs:label": {
        "@value": "planned within",
        "@language": "en"
      },
      "rdfs:domain": {
        "owl:unionOf": {
          "@list": [
            {
              "@id": "vf:Process"
            },
            {
              "@id": "vf:Commitment"
            },
            {
              "@id": "vf:Intent"
            }
          ]
        }
      },
      "rdfs:range": {
        "@id": "vf:Plan"
      },
      "vs:term_status": "testing",
      "rdfs:comment": {
        "@value": "The non-process commitment/intent or process with its inputs and outputs is part of the plan.",
        "@language": "en"
      }
    },
    {
      "@id": "vf:planIncludes",
      "@type": "owl:ObjectProperty",
      "owl:inverseOf": {
        "@id": "vf:plannedWithin"
      },
      "rdfs:label": {
        "@value": "plan includes",
        "@language": "en"
      },
      "rdfs:domain": {
        "@id": "vf:Plan"
      },
      "rdfs:range": {
        "owl:unionOf": {
          "@list": [
            {
              "@id": "vf:Process"
            },
            {
              "@id": "vf:Commitment"
            },
            {
              "@id": "vf:Intent"
            }
          ]
        }
      },
      "vs:term_status": "unstable",
      "rdfs:comment": {
        "@value": "The processes and and non-process commitments/intents that constitute the plan.",
        "@language": "en"
      }
    },
    {
      "@id": "vf:independentDemandOf",
      "@type": "owl:ObjectProperty",
      "rdfs:label": {
        "@value": "independent demand of",
        "@language": "en"
      },
      "rdfs:range": {
        "@id": "vf:Plan"
      },
      "rdfs:domain": {
        "owl:unionOf": {
          "@list": [
            {
              "@id": "vf:Commitment"
            },
            {
              "@id": "vf:Intent"
            }
          ]
        }
      },
      "vs:term_status": "testing",
      "rdfs:comment": {
        "@value": "This plan is the way this commitment or intent will be realized.",
        "@language": "en"
      }
    },
    {
      "@id": "vf:hasIndependentDemand",
      "@type": "owl:ObjectProperty",
      "owl:inverseOf": {
        "@id": "vf:independentDemandOf"
      },
      "rdfs:label": {
        "@value": "has independent demand",
        "@language": "en"
      },
      "rdfs:range": {
        "owl:unionOf": {
          "@list": [
            {
              "@id": "vf:Commitment"
            },
            {
              "@id": "vf:Intent"
            }
          ]
        }
      },
      "rdfs:domain": {
        "@id": "vf:Plan"
      },
      "vs:term_status": "testing",
      "rdfs:comment": {
        "@value": "The commitments and/or intents which this plan was created to deliver.",
        "@language": "en"
      }
    },
    {
      "@id": "vf:resourceInventoriedAs",
      "@type": "owl:ObjectProperty",
      "rdfs:label": {
        "@value": "resource inventoried as",
        "@language": "en"
      },
      "rdfs:domain": {
        "owl:unionOf": {
          "@list": [
            {
              "@id": "vf:Commitment"
            },
            {
              "@id": "vf:Intent"
            },
            {
              "@id": "vf:EconomicEvent"
            }
          ]
        }
      },
      "rdfs:range": {
        "@id": "vf:EconomicResource"
      },
      "vs:term_status": "stable",
      "rdfs:comment": {
        "@value": "Economic resource involved in the flow.",
        "@language": "en"
      }
    },
    {
      "@id": "vf:toResourceInventoriedAs",
      "@type": "owl:ObjectProperty",
      "rdfs:label": {
        "@value": "to resource inventoried as",
        "@language": "en"
      },
      "rdfs:domain": {
        "@id": "vf:EconomicEvent"
      },
      "rdfs:range": {
        "@id": "vf:EconomicResource"
      },
      "vs:term_status": "testing",
      "rdfs:comment": {
        "@value": "Additional economic resource on the economic event when needed by the receiver. Used when a transfer or move, or sometimes other actions, requires explicitly identifying an economic resource on the receiving side.",
        "@language": "en"
      }
    },
    {
      "@id": "vf:relationship",
      "@type": "owl:ObjectProperty",
      "rdfs:label": {
        "@value": "relationship",
        "@language": "en"
      },
      "rdfs:domain": {
        "@id": "vf:AgentRelationship"
      },
      "rdfs:range": {
        "@id": "vf:AgentRelationshipRole"
      },
      "vs:term_status": "stable",
      "rdfs:comment": {
        "@value": "The role of an economic relationship that exists between 2 agents, such as member, trading partner.",
        "@language": "en"
      }
    },
    {
      "@id": "vf:appreciationOf",
      "@type": "owl:ObjectProperty",
      "rdfs:label": {
        "@value": "appreciation of",
        "@language": "en"
      },
      "rdfs:domain": {
        "@id": "vf:Appreciation"
      },
      "rdfs:range": {
        "@id": "vf:EconomicEvent"
      },
      "vs:term_status": "unstable",
      "rdfs:comment": {
        "@value": "The economic event being appreciated (gift economy).",
        "@language": "en"
      }
    },
    {
      "@id": "vf:appreciationWith",
      "@type": "owl:ObjectProperty",
      "rdfs:label": {
        "@value": "appreciation with",
        "@language": "en"
      },
      "rdfs:domain": {
        "@id": "vf:Appreciation"
      },
      "rdfs:range": {
        "@id": "vf:EconomicEvent"
      },
      "vs:term_status": "unstable",
      "rdfs:comment": {
        "@value": "The economic event implemented in appreciation (gift economy).",
        "@language": "en"
      }
    },
    {
      "@id": "vf:provider",
      "@type": "owl:ObjectProperty",
      "rdfs:domain": {
        "owl:unionOf": {
          "@list": [
            {
              "@id": "vf:EconomicEvent"
            },
            {
              "@id": "vf:Commitment"
            },
            {
              "@id": "vf:Intent"
            },
            {
              "@id": "vf:Claim"
            }
          ]
        }
      },
      "rdfs:label": {
        "@value": "provider",
        "@language": "en"
      },
      "rdfs:range": {
        "@id": "vf:Agent"
      },
      "vs:term_status": "stable",
      "rdfs:comment": {
        "@value": "The economic agent from whom the intended, committed, or actual economic event is initiated.",
        "@language": "en"
      }
    },
    {
      "@id": "vf:receiver",
      "@type": "owl:ObjectProperty",
      "rdfs:domain": {
        "owl:unionOf": {
          "@list": [
            {
              "@id": "vf:EconomicEvent"
            },
            {
              "@id": "vf:Commitment"
            },
            {
              "@id": "vf:Intent"
            },
            {
              "@id": "vf:Claim"
            }
          ]
        }
      },
      "rdfs:label": {
        "@value": "receiver",
        "@language": "en"
      },
      "rdfs:range": {
        "@id": "vf:Agent"
      },
      "vs:term_status": "stable",
      "rdfs:comment": {
        "@value": "The economic agent whom the intended, committed, or actual economic event is for.",
        "@language": "en"
      }
    },
    {
      "@id": "vf:subject",
      "@type": "owl:ObjectProperty",
      "rdfs:domain": {
        "@id": "vf:AgentRelationship"
      },
      "rdfs:label": {
        "@value": "subject",
        "@language": "en"
      },
      "rdfs:range": {
        "@id": "vf:Agent"
      },
      "vs:term_status": "stable",
      "rdfs:comment": {
        "@value": "The subject of a relationship between 2 agents.  For example, if Mary is a member of a group, then Mary is the subject.",
        "@language": "en"
      }
    },
    {
      "@id": "vf:object",
      "@type": "owl:ObjectProperty",
      "rdfs:domain": {
        "@id": "vf:AgentRelationship"
      },
      "rdfs:label": {
        "@value": "object",
        "@language": "en"
      },
      "rdfs:range": {
        "@id": "vf:Agent"
      },
      "vs:term_status": "stable",
      "rdfs:comment": {
        "@value": "The object of a relationship between 2 agents.  For example, if Mary is a member of a group, then the group is the object.",
        "@language": "en"
      }
    },
    {
      "@id": "vf:inScopeOf",
      "@type": "owl:ObjectProperty",
      "rdfs:domain": {
        "owl:unionOf": {
          "@list": [
            {
              "@id": "vf:Claim"
            },
            {
              "@id": "vf:Commitment"
            },
            {
              "@id": "vf:EconomicEvent"
            },
            {
              "@id": "vf:Proposal"
            },
            {
              "@id": "vf:Intent"
            },
            {
              "@id": "vf:Scenario"
            },
            {
              "@id": "vf:Process"
            },
            {
              "@id": "vf:AgentRelationship"
            }
          ]
        }
      },
      "rdfs:label": {
        "@value": "in scope of",
        "@language": "en"
      },
      "rdfs:range": {
        "@id": "vf:Agent"
      },
      "vs:term_status": "unstable",
      "rdfs:comment": {
        "@value": "In the context of an agent, a grouping generally used for accounting, reporting.",
        "@language": "en"
      }
    },
    {
      "@id": "vf:triggeredBy",
      "@type": "owl:ObjectProperty",
      "rdfs:label": {
        "@value": "triggered by",
        "@language": "en"
      },
      "rdfs:domain": {
        "owl:unionOf": {
          "@list": [
            {
              "@id": "vf:EconomicEvent"
            },
            {
              "@id": "vf:Claim"
            }
          ]
        }
      },
      "rdfs:range": {
        "@id": "vf:EconomicEvent"
      },
      "vs:term_status": "unstable",
      "rdfs:comment": {
        "@value": "References an economic event that implied the claim or event, often based on a prior agreement.",
        "@language": "en"
      }
    },
    {
      "@id": "vf:corrects",
      "@type": "owl:ObjectProperty",
      "rdfs:label": {
        "@value": "corrects",
        "@language": "en"
      },
      "rdfs:domain": {
        "@id": "vf:EconomicEvent"
      },
      "rdfs:range": {
        "@id": "vf:EconomicEvent"
      },
      "vs:term_status": "unstable",
      "rdfs:comment": {
        "@value": "Used when an event was entered incorrectly and needs to be backed out or corrected. (The initial event cannot be changed.)",
        "@language": "en"
      }
    },
    {
      "@id": "vf:settles",
      "@type": "owl:ObjectProperty",
      "rdfs:label": {
        "@value": "settles",
        "@language": "en"
      },
      "rdfs:domain": {
        "@id": "vf:EconomicEvent"
      },
      "rdfs:range": {
        "@id": "vf:Claim"
      },
      "vs:term_status": "unstable",
      "rdfs:comment": {
        "@value": "References a claim that is fully or partially settled by the economic event.",
        "@language": "en"
      }
    },
    {
      "@id": "vf:containedIn",
      "@type": "owl:ObjectProperty",
      "rdfs:label": {
        "@value": "contained in",
        "@language": "en"
      },
      "rdfs:domain": {
        "@id": "vf:EconomicResource"
      },
      "rdfs:range": {
        "@id": "vf:EconomicResource"
      },
      "vs:term_status": "unstable",
      "rdfs:comment": {
        "@value": "Used when a stock economic resource contains units also defined as economic resources.",
        "@language": "en"
      }
    },
    {
      "@id": "vf:primaryAccountable",
      "@type": "owl:ObjectProperty",
      "rdfs:label": {
        "@value": "primary accountable",
        "@language": "en"
      },
      "rdfs:domain": {
        "@id": "vf:EconomicResource"
      },
      "rdfs:range": {
        "@id": "vf:Agent"
      },
      "vs:term_status": "testing",
      "rdfs:comment": {
        "@value": "The agent currently with primary rights and responsibilites for the economic resource. It is the agent that is associated with the accountingQuantity of the economic resource.",
        "@language": "en"
      }
    },
    {
      "@id": "vf:hasBeginning",
      "@type": "owl:DatatypeProperty",
      "rdfs:label": {
        "@value": "has beginning",
        "@language": "en"
      },
      "rdfs:domain": [
        {
          "@id": "time:TemporalEntity"
        },
        {
          "owl:unionOf": {
            "@list": [
              {
                "@id": "vf:Commitment"
              },
              {
                "@id": "vf:EconomicEvent"
              },
              {
                "@id": "vf:Intent"
              },
              {
                "@id": "vf:Proposal"
              },
              {
                "@id": "vf:Scenario"
              },
              {
                "@id": "vf:Process"
              }
            ]
          }
        }
      ],
      "rdfs:range": {
        "@id": "xsd:dateTimeStamp"
      },
      "vs:term_status": "testing",
      "owl:propertyChainAxiom": {
        "@list": [
          {
            "@id": "time:hasBeginning"
          },
          {
            "@id": "time:inXSDDateTimeStamp"
          }
        ]
      },
      "rdfs:comment": {
        "@value": "The planned or actual beginning of a flow or process.",
        "@language": "en"
      }
    },
    {
      "@id": "vf:hasEnd",
      "@type": "owl:DatatypeProperty",
      "rdfs:label": {
        "@value": "has end",
        "@language": "en"
      },
      "rdfs:domain": [
        {
          "@id": "time:TemporalEntity"
        },
        {
          "owl:unionOf": {
            "@list": [
              {
                "@id": "vf:Commitment"
              },
              {
                "@id": "vf:EconomicEvent"
              },
              {
                "@id": "vf:Intent"
              },
              {
                "@id": "vf:Proposal"
              },
              {
                "@id": "vf:Scenario"
              },
              {
                "@id": "vf:Process"
              }
            ]
          }
        }
      ],
      "rdfs:range": {
        "@id": "xsd:dateTimeStamp"
      },
      "vs:term_status": "testing",
      "owl:propertyChainAxiom": {
        "@list": [
          {
            "@id": "time:hasEnd"
          },
          {
            "@id": "time:inXSDDateTimeStamp"
          }
        ]
      },
      "rdfs:comment": {
        "@value": "The planned or actual end of a flow or process.",
        "@language": "en"
      }
    },
    {
      "@id": "vf:hasPointInTime",
      "@type": "owl:DatatypeProperty",
      "rdfs:label": {
        "@value": "has point in time",
        "@language": "en"
      },
      "rdfs:domain": [
        {
          "@id": "time:Instant"
        },
        {
          "owl:unionOf": {
            "@list": [
              {
                "@id": "vf:Commitment"
              },
              {
                "@id": "vf:EconomicEvent"
              },
              {
                "@id": "vf:Intent"
              }
            ]
          }
        }
      ],
      "rdfs:range": {
        "@id": "xsd:dateTimeStamp"
      },
      "vs:term_status": "testing",
      "owl:propertyChainAxiom": {
        "@list": [
          {
            "@id": "time:hasEnd"
          },
          {
            "@id": "time:inXSDDateTimeStamp"
          }
        ]
      },
      "rdfs:comment": {
        "@value": "The planned or actual time of a flow; can be used instead of hasBeginning and hasEnd, if so, hasBeginning and hasEnd should be able to be returned with this value.",
        "@language": "en"
      }
    },
    {
      "@id": "time:hasDuration",
      "rdfs:label": {
        "@value": "has duration",
        "@language": "en"
      },
      "rdfs:domain": {
        "owl:unionOf": {
          "@list": [
            {
              "@id": "vf:RecipeProcess"
            },
            {
              "@id": "vf:ScenarioDefinition"
            }
          ]
        }
      }
    },
    {
      "@id": "vf:due",
      "@type": "owl:DatatypeProperty",
      "rdfs:label": {
        "@value": "due",
        "@language": "en"
      },
      "rdfs:domain": {
        "owl:unionOf": {
          "@list": [
            {
              "@id": "vf:Plan"
            },
            {
              "@id": "vf:Commitment"
            },
            {
              "@id": "vf:Claim"
            },
            {
              "@id": "vf:Intent"
            }
          ]
        }
      },
      "rdfs:range": {
        "@id": "xsd:dateTimeStamp"
      },
      "vs:term_status": "testing",
      "rdfs:comment": {
        "@value": "The time something is expected to be complete.",
        "@language": "en"
      }
    },
    {
      "@id": "vf:localLabel",
      "@type": "owl:DatatypeProperty",
      "rdfs:label": {
        "@value": "unit local label",
        "@language": "en"
      },
      "rdfs:domain": {
        "@id": "om2:Unit"
      },
      "rdfs:range": {
        "@id": "xsd:string"
      },
      "vs:term_status": "unstable",
      "rdfs:comment": {
        "@value": "An override label to optionally display for units of measure.",
        "@language": "en"
      }
    },
    {
      "@id": "vf:localSymbol",
      "@type": "owl:DatatypeProperty",
      "rdfs:label": {
        "@value": "unit local symbol",
        "@language": "en"
      },
      "rdfs:domain": {
        "@id": "om2:Unit"
      },
      "rdfs:range": {
        "@id": "xsd:string"
      },
      "vs:term_status": "unstable",
      "rdfs:comment": {
        "@value": "An override symbol to optionally display for units of measure.",
        "@language": "en"
      }
    },
    {
      "@id": "vf:accountingQuantity",
      "@type": "owl:ObjectProperty",
      "rdfs:label": {
        "@value": "accounting quantity",
        "@language": "en"
      },
      "rdfs:domain": {
        "@id": "vf:EconomicResource"
      },
      "rdfs:range": {
        "@id": "om2:Measure"
      },
      "vs:term_status": "testing",
      "rdfs:comment": {
        "@value": "The current amount and unit of the economic resource for which the agent has primary rights and responsibilities, sometimes thought of as ownership. This can be either stored or derived from economic events affecting the resource.",
        "@language": "en"
      }
    },
    {
      "@id": "vf:onhandQuantity",
      "@type": "owl:ObjectProperty",
      "rdfs:label": {
        "@value": "onhand quantity",
        "@language": "en"
      },
      "rdfs:domain": {
        "@id": "vf:EconomicResource"
      },
      "rdfs:range": {
        "@id": "om2:Measure"
      },
      "vs:term_status": "testing",
      "rdfs:comment": {
        "@value": "The current amount and unit of the economic resource which is under direct control of the agent.  It may be more or less than the accounting quantity. This can be either stored or derived from economic events affecting the resource.",
        "@language": "en"
      }
    },
    {
      "@id": "vf:resourceQuantity",
      "@type": "owl:ObjectProperty",
      "rdfs:label": {
        "@value": "resource quantity",
        "@language": "en"
      },
      "rdfs:domain": {
        "owl:unionOf": {
          "@list": [
            {
              "@id": "vf:EconomicEvent"
            },
            {
              "@id": "vf:Commitment"
            },
            {
              "@id": "vf:Intent"
            },
            {
              "@id": "vf:RecipeFlow"
            },
            {
              "@id": "vf:Claim"
            }
          ]
        }
      },
      "rdfs:range": {
        "@id": "om2:Measure"
      },
      "vs:term_status": "stable",
      "rdfs:comment": {
        "@value": "The amount and unit of the economic resource counted or inventoried.",
        "@language": "en"
      }
    },
    {
      "@id": "vf:effortQuantity",
      "@type": "owl:ObjectProperty",
      "rdfs:label": {
        "@value": "effort quantity",
        "@language": "en"
      },
      "rdfs:domain": {
        "owl:unionOf": {
          "@list": [
            {
              "@id": "vf:EconomicEvent"
            },
            {
              "@id": "vf:Commitment"
            },
            {
              "@id": "vf:Intent"
            },
            {
              "@id": "vf:RecipeFlow"
            },
            {
              "@id": "vf:Claim"
            }
          ]
        }
      },
      "rdfs:range": {
        "@id": "om2:Measure"
      },
      "vs:term_status": "testing",
      "rdfs:comment": {
        "@value": "The amount and unit of the work or use or citation effort-based action. This is often a time duration, but also could be cycle counts or other measures of effort or usefulness.",
        "@language": "en"
      }
    },
    {
      "@id": "vf:availableQuantity",
      "@type": "owl:ObjectProperty",
      "rdfs:label": {
        "@value": "available quantity",
        "@language": "en"
      },
      "rdfs:domain": {
        "@id": "vf:Intent"
      },
      "rdfs:range": {
        "@id": "om2:Measure"
      },
      "vs:term_status": "testing",
      "rdfs:comment": {
        "@value": "The quantity of the offered resource currently available.",
        "@language": "en"
      }
    },
    {
      "@id": "vf:minimumQuantity",
      "@type": "owl:ObjectProperty",
      "rdfs:label": {
        "@value": "minimum quantity",
        "@language": "en"
      },
      "rdfs:domain": {
        "@id": "vf:Intent"
      },
      "rdfs:range": {
        "@id": "om2:Measure"
      },
      "vs:term_status": "testing",
      "rdfs:comment": {
        "@value": "The minimum required order quantity of the offered resource.",
        "@language": "en"
      }
    },
    {
      "@id": "om2:hasNumericalValue",
      "rdfs:range": {
        "@id": "dtype:numericUnion"
      }
    },
    {
      "@id": "vf:unitBased",
      "@type": "owl:DatatypeProperty",
      "rdfs:label": {
        "@value": "unit based",
        "@language": "en"
      },
      "rdfs:domain": {
        "@id": "vf:Proposal"
      },
      "rdfs:range": {
        "@id": "xsd:boolean"
      },
      "vs:term_status": "testing",
      "rdfs:comment": {
        "@value": "This proposal contains unit based quantities, which can be multipied to create commitments; commonly seen in a price list or e-commerce.",
        "@language": "en"
      }
    },
    {
      "@id": "vf:purpose",
      "@type": "owl:ObjectProperty",
      "rdfs:label": {
        "@value": "purpose",
        "@language": "en"
      },
      "rdfs:domain": {
        "@id": "vf:Proposal"
      },
      "rdfs:range": {
        "@id": "vf:ProposalPurpose"
      },
      "vs:term_status": "testing",
      "rdfs:comment": {
        "@value": "The type of proposal, offer or request.",
        "@language": "en"
      }
    },
    {
      "@id": "dcterms:created",
      "rdfs:domain": {
        "owl:unionOf": {
          "@list": [
            {
              "@id": "vf:Agreement"
            },
            {
              "@id": "vf:Claim"
            },
            {
              "@id": "vf:Commitment"
            },
            {
              "@id": "vf:Plan"
            },
            {
              "@id": "vf:Proposal"
            },
            {
              "@id": "vf:EconomicEvent"
            }
          ]
        }
      }
    },
    {
      "@id": "geo:long",
      "rdfs:range": {
        "@id": "xsd:double"
      }
    },
    {
      "@id": "geo:lat",
      "rdfs:range": {
        "@id": "xsd:double"
      }
    },
    {
      "@id": "geo:alt",
      "rdfs:range": {
        "@id": "xsd:double"
      }
    },
    {
      "@id": "vf:currentLocation",
      "@type": "owl:ObjectProperty",
      "rdfs:label": {
        "@value": "current location",
        "@language": "en"
      },
      "rdfs:domain": {
        "@id": "vf:EconomicResource"
      },
      "rdfs:range": {
        "@id": "geo:SpatialThing"
      },
      "vs:term_status": "unstable",
      "rdfs:comment": {
        "@value": "The current place an economic resource is located.  Could be at any level of granularity, from a town to an address to a warehouse location.  Usually mappable.",
        "@language": "en"
      }
    },
    {
      "@id": "vf:currentVirtualLocation",
      "@type": "owl:DatatypeProperty",
      "rdfs:label": {
        "@value": "current virtual location",
        "@language": "en"
      },
      "rdfs:domain": {
        "@id": "vf:EconomicResource"
      },
      "rdfs:range": {
        "@id": "xsd:anyURI"
      },
      "vs:term_status": "unstable",
      "rdfs:comment": {
        "@value": "The current virtual place an electronic economic resource is located.",
        "@language": "en"
      }
    },
    {
      "@id": "vf:primaryLocation",
      "@type": "owl:ObjectProperty",
      "rdfs:label": {
        "@value": "primary location",
        "@language": "en"
      },
      "rdfs:domain": {
        "@id": "vf:Agent"
      },
      "rdfs:range": {
        "@id": "geo:SpatialThing"
      },
      "vs:term_status": "unstable",
      "rdfs:comment": {
        "@value": "The main place an agent is located, often an address where activities occur and mail can be sent. This is usually a mappable geographic location.  It also could be a website address, as in the case of agents who have no physical location.",
        "@language": "en"
      }
    },
    {
      "@id": "vf:eligibleLocation",
      "@type": "owl:ObjectProperty",
      "rdfs:label": {
        "@value": "eligible location",
        "@language": "en"
      },
      "rdfs:domain": {
        "@id": "vf:Proposal"
      },
      "rdfs:range": {
        "@id": "geo:SpatialThing"
      },
      "vs:term_status": "unstable",
      "rdfs:comment": {
        "@value": "Location or area where the proposal is valid.",
        "@language": "en"
      }
    },
    {
      "@id": "vf:atLocation",
      "@type": "owl:ObjectProperty",
      "rdfs:label": {
        "@value": "at location",
        "@language": "en"
      },
      "rdfs:domain": {
        "owl:unionOf": {
          "@list": [
            {
              "@id": "vf:EconomicEvent"
            },
            {
              "@id": "vf:Commitment"
            },
            {
              "@id": "vf:Intent"
            }
          ]
        }
      },
      "rdfs:range": {
        "@id": "geo:SpatialThing"
      },
      "vs:term_status": "unstable",
      "rdfs:comment": {
        "@value": "The place where an intent, commitment, or economic event occurs.  Usually mappable.",
        "@language": "en"
      }
    },
    {
      "@id": "vf:toLocation",
      "@type": "owl:ObjectProperty",
      "rdfs:label": {
        "@value": "to location",
        "@language": "en"
      },
      "rdfs:domain": {
        "@id": "vf:EconomicEvent"
      },
      "rdfs:range": {
        "@id": "geo:SpatialThing"
      },
      "vs:term_status": "unstable",
      "rdfs:comment": {
        "@value": "The new location of the receiver resource.",
        "@language": "en"
      }
    },
    {
      "@id": "vf:image",
      "@type": "owl:DatatypeProperty",
      "rdfs:label": {
        "@value": "image",
        "@language": "en"
      },
      "rdfs:domain": {
        "owl:unionOf": {
          "@list": [
            {
              "@id": "vf:Agent"
            },
            {
              "@id": "vf:EconomicEvent"
            },
            {
              "@id": "vf:EconomicResource"
            },
            {
              "@id": "vf:Intent"
            },
            {
              "@id": "vf:ResourceSpecification"
            },
            {
              "@id": "vf:ProcessSpecification"
            },
            {
              "@id": "vf:RecipeProcess"
            }
          ]
        }
      },
      "rdfs:range": {
        "@id": "xsd:anyURI"
      },
      "vs:term_status": "testing",
      "rdfs:comment": {
        "@value": "The uri to an image relevant to the entity, such as a logo, avatar, photo, diagram, etc.",
        "@language": "en"
      }
    },
    {
      "@id": "vf:imageList",
      "@type": "owl:DatatypeProperty",
      "rdfs:label": {
        "@value": "image list",
        "@language": "en"
      },
      "rdfs:domain": {
        "owl:unionOf": {
          "@list": [
            {
              "@id": "vf:EconomicResource"
            },
            {
              "@id": "vf:Intent"
            },
            {
              "@id": "vf:ResourceSpecification"
            }
          ]
        }
      },
      "rdfs:range": {
        "@id": "xsd:anyURI"
      },
      "vs:term_status": "testing",
      "rdfs:comment": {
        "@value": "A comma separated list of uri addresses to images relevant to the resource.",
        "@language": "en"
      }
    },
    {
      "@id": "vf:name",
      "@type": "owl:DatatypeProperty",
      "rdfs:label": {
        "@value": "name",
        "@language": "en"
      },
      "rdfs:range": {
        "@id": "xsd:string"
      },
      "rdfs:domain": {
        "owl:unionOf": {
          "@list": [
            {
              "@id": "geo:SpatialThing"
            },
            {
              "@id": "vf:Agent"
            },
            {
              "@id": "vf:Agreement"
            },
            {
              "@id": "vf:EconomicResource"
            },
            {
              "@id": "vf:Plan"
            },
            {
              "@id": "vf:Process"
            },
            {
              "@id": "vf:ProcessSpecification"
            },
            {
              "@id": "vf:Proposal"
            },
            {
              "@id": "vf:Recipe"
            },
            {
              "@id": "vf:RecipeGroup"
            },
            {
              "@id": "vf:RecipeProcess"
            },
            {
              "@id": "vf:ResourceSpecification"
            },
            {
              "@id": "vf:RoleBehavior"
            },
            {
              "@id": "vf:Scenario"
            },
            {
              "@id": "vf:ScenarioDefinition"
            }
          ]
        }
      },
      "vs:term_status": "testing",
      "rdfs:comment": {
        "@value": "An informal or formal textual identifier for an object. Does not imply uniqueness.",
        "@language": "en"
      }
    },
    {
      "@id": "skos:note",
      "rdfs:domain": {
        "owl:unionOf": {
          "@list": [
            {
              "@id": "geo:SpatialThing"
            },
            {
              "@id": "vf:Agent"
            },
            {
              "@id": "vf:AgentRelationship"
            },
            {
              "@id": "vf:AgentRelationshipRole"
            },
            {
              "@id": "vf:Agreement"
            },
            {
              "@id": "vf:Appreciation"
            },
            {
              "@id": "vf:Claim"
            },
            {
              "@id": "vf:Commitment"
            },
            {
              "@id": "vf:EconomicEvent"
            },
            {
              "@id": "vf:EconomicResource"
            },
            {
              "@id": "vf:ExternalLink"
            },
            {
              "@id": "vf:Intent"
            },
            {
              "@id": "vf:Plan"
            },
            {
              "@id": "vf:Process"
            },
            {
              "@id": "vf:ProcessSpecification"
            },
            {
              "@id": "vf:Proposal"
            },
            {
              "@id": "vf:Recipe"
            },
            {
              "@id": "vf:RecipeFlow"
            },
            {
              "@id": "vf:RecipeGroup"
            },
            {
              "@id": "vf:RecipeProcess"
            },
            {
              "@id": "vf:ResourceSpecification"
            },
            {
              "@id": "vf:RoleBehavior"
            },
            {
              "@id": "vf:Scenario"
            },
            {
              "@id": "vf:ScenarioDefinition"
            }
          ]
        }
      }
    },
    {
      "@id": "vf:trackingIdentifier",
      "@type": "owl:DatatypeProperty",
      "rdfs:label": {
        "@value": "tracking identifier",
        "@language": "en"
      },
      "rdfs:domain": {
        "@id": "vf:EconomicResource"
      },
      "rdfs:range": {
        "@id": "xsd:string"
      },
      "vs:term_status": "testing",
      "rdfs:comment": {
        "@value": "Any identifier used to track the resource, such as a serial number or VIN or lot/batch identifier.",
        "@language": "en"
      }
    },
    {
      "@id": "vf:expiresOn",
      "@type": "owl:DatatypeProperty",
      "rdfs:label": {
        "@value": "expires on",
        "@language": "en"
      },
      "rdfs:domain": {
        "@id": "vf:EconomicResource"
      },
      "rdfs:range": {
        "@id": "xsd:dateTimeStamp"
      },
      "vs:term_status": "unstable",
      "rdfs:comment": {
        "@value": "If the resource is being tracked as a lot or batch, this is the date the batch expires, after which it is not recommended to use/consume.",
        "@language": "en"
      }
    },
    {
      "@id": "vf:fulfills",
      "@type": "owl:ObjectProperty",
      "rdfs:label": {
        "@value": "fulfills",
        "@language": "en"
      },
      "rdfs:domain": {
        "@id": "vf:EconomicEvent"
      },
      "rdfs:range": {
        "@id": "vf:Commitment"
      },
      "vs:term_status": "testing",
      "rdfs:comment": {
        "@value": "The commitment which is completely or partially fulfilled by an economic event.",
        "@language": "en"
      }
    },
    {
      "@id": "vf:satisfies",
      "@type": "owl:ObjectProperty",
      "rdfs:label": {
        "@value": "satisfies",
        "@language": "en"
      },
      "rdfs:domain": {
        "owl:unionOf": {
          "@list": [
            {
              "@id": "vf:Commitment"
            },
            {
              "@id": "vf:EconomicEvent"
            }
          ]
        }
      },
      "rdfs:range": {
        "@id": "vf:Intent"
      },
      "vs:term_status": "testing",
      "rdfs:comment": {
        "@value": "An intent satisfied fully or partially by an economic event or commitment.",
        "@language": "en"
      }
    },
    {
      "@id": "vf:publishes",
      "@type": "owl:ObjectProperty",
      "rdfs:label": {
        "@value": "publishes",
        "@language": "en"
      },
      "rdfs:domain": {
        "@id": "vf:Proposal"
      },
      "rdfs:range": {
        "@id": "vf:Intent"
      },
      "vs:term_status": "testing",
      "rdfs:comment": {
        "@value": "The primary intent(s) of this published proposal. Would be used in intent matching.",
        "@language": "en"
      }
    },
    {
      "@id": "vf:reciprocal",
      "@type": "owl:ObjectProperty",
      "rdfs:label": {
        "@value": "reciprocal",
        "@language": "en"
      },
      "rdfs:domain": {
        "@id": "vf:Proposal"
      },
      "rdfs:range": {
        "@id": "vf:Intent"
      },
      "vs:term_status": "testing",
      "rdfs:comment": {
        "@value": "The reciprocal intent(s) of this published proposal. Not meant to be used for intent matching.",
        "@language": "en"
      }
    },
    {
      "@id": "vf:proposedTo",
      "@type": "owl:ObjectProperty",
      "rdfs:label": {
        "@value": "proposed to",
        "@language": "en"
      },
      "rdfs:domain": {
        "@id": "vf:Proposal"
      },
      "rdfs:range": {
        "@id": "vf:Agent"
      },
      "vs:term_status": "unstable",
      "rdfs:comment": {
        "@value": "The agent(s) to which the proposal is published.",
        "@language": "en"
      }
    },
    {
      "@id": "vf:listedIn",
      "@type": "owl:ObjectProperty",
      "rdfs:label": {
        "@value": "listed in",
        "@language": "en"
      },
      "rdfs:domain": {
        "@id": "vf:Proposal"
      },
      "rdfs:range": {
        "@id": "vf:ProposalList"
      },
      "vs:term_status": "unstable",
      "rdfs:comment": {
        "@value": "This proposal is part of a list of proposals.",
        "@language": "en"
      }
    },
    {
      "@id": "vf:lists",
      "@type": "owl:ObjectProperty",
      "owl:inverseOf": {
        "@id": "vf:listedIn"
      },
      "rdfs:label": {
        "@value": "lists",
        "@language": "en"
      },
      "rdfs:domain": {
        "@id": "vf:ProposalList"
      },
      "rdfs:range": {
        "@id": "vf:Proposal"
      },
      "vs:term_status": "unstable",
      "rdfs:comment": {
        "@value": "All the proposals included in this proposal list.",
        "@language": "en"
      }
    },
    {
      "@id": "vf:finished",
      "@type": "owl:DatatypeProperty",
      "rdfs:domain": {
        "owl:unionOf": {
          "@list": [
            {
              "@id": "vf:Commitment"
            },
            {
              "@id": "vf:Process"
            },
            {
              "@id": "vf:Intent"
            },
            {
              "@id": "vf:Claim"
            }
          ]
        }
      },
      "rdfs:label": {
        "@value": "finished",
        "@language": "en"
      },
      "rdfs:range": {
        "@id": "xsd:boolean"
      },
      "vs:term_status": "stable",
      "rdfs:comment": {
        "@value": "The commitment or intent or process is complete or not.  This is irrespective of if the original goal has been met, and indicates that no more will be done.",
        "@language": "en"
      }
    },
    {
      "@id": "vf:substitutable",
      "@type": "owl:DatatypeProperty",
      "rdfs:label": {
        "@value": "substitutable",
        "@language": "en"
      },
      "rdfs:domain": {
        "@id": "vf:ResourceSpecification"
      },
      "rdfs:range": {
        "@id": "xsd:boolean"
      },
      "vs:term_status": "testing",
      "rdfs:comment": {
        "@value": "Defines if any resource of that type can be freely substituted for any other resource of that type when used, consumed, traded, etc.",
        "@language": "en"
      }
    },
    {
      "@id": "vf:unitOfEffort",
      "@type": "owl:ObjectProperty",
      "rdfs:label": {
        "@value": "unit of effort",
        "@language": "en"
      },
      "rdfs:domain": {
        "@id": "vf:EconomicResource"
      },
      "rdfs:range": {
        "@id": "om2:Unit"
      },
      "vs:term_status": "unstable",
      "rdfs:comment": {
        "@value": "The unit used for use or work or sometimes cite actions.",
        "@language": "en"
      }
    },
    {
      "@id": "vf:defaultUnitOfEffort",
      "@type": "owl:ObjectProperty",
      "rdfs:label": {
        "@value": "default unit of effort",
        "@language": "en"
      },
      "rdfs:domain": {
        "@id": "vf:ResourceSpecification"
      },
      "rdfs:range": {
        "@id": "om2:Unit"
      },
      "vs:term_status": "testing",
      "rdfs:comment": {
        "@value": "The default unit used for use or work.",
        "@language": "en"
      }
    },
    {
      "@id": "vf:defaultUnitOfResource",
      "@type": "owl:ObjectProperty",
      "rdfs:label": {
        "@value": "default unit of resource",
        "@language": "en"
      },
      "rdfs:domain": {
        "@id": "vf:ResourceSpecification"
      },
      "rdfs:range": {
        "@id": "om2:Unit"
      },
      "vs:term_status": "testing",
      "rdfs:comment": {
        "@value": "The default unit used for the resource itself.",
        "@language": "en"
      }
    },
    {
      "@id": "vf:basedOn",
      "@type": "owl:ObjectProperty",
      "rdfs:label": {
        "@value": "based on",
        "@language": "en"
      },
      "rdfs:domain": {
        "@id": "vf:Process"
      },
      "rdfs:range": {
        "@id": "vf:ProcessSpecification"
      },
      "vs:term_status": "testing",
      "rdfs:comment": {
        "@value": "The definition or standard specification for a process.",
        "@language": "en"
      }
    },
    {
      "@id": "vf:classifiedAs",
      "@type": "owl:ObjectProperty",
      "rdfs:label": {
        "@value": "classified as",
        "@language": "en"
      },
      "rdfs:domain": {
        "owl:unionOf": {
          "@list": [
            {
              "@id": "vf:Process"
            },
            {
              "@id": "vf:EconomicResource"
            },
            {
              "@id": "vf:Organization"
            },
            {
              "@id": "vf:EcologicalAgent"
            }
          ]
        }
      },
      "rdfs:range": {
        "@id": "owl:Thing"
      },
      "vs:term_status": "unstable",
      "rdfs:comment": {
        "@value": "References one or more concepts in a common taxonomy or other classification scheme for purposes of categorization or grouping.",
        "@language": "en"
      }
    },
    {
      "@id": "vf:resourceClassifiedAs",
      "@type": "owl:ObjectProperty",
      "rdfs:label": {
        "@value": "resource classified as",
        "@language": "en"
      },
      "rdfs:domain": {
        "owl:unionOf": {
          "@list": [
            {
              "@id": "vf:ResourceSpecification"
            },
            {
              "@id": "vf:RecipeFlow"
            },
            {
              "@id": "vf:Intent"
            },
            {
              "@id": "vf:Commitment"
            },
            {
              "@id": "vf:EconomicEvent"
            },
            {
              "@id": "vf:Claim"
            }
          ]
        }
      },
      "rdfs:range": {
        "@id": "owl:Thing"
      },
      "vs:term_status": "unstable",
      "rdfs:comment": {
        "@value": "References a concept in a common taxonomy or other classification scheme for purposes of categorization or grouping.",
        "@language": "en"
      }
    },
    {
      "@id": "vf:processClassifiedAs",
      "@type": "owl:ObjectProperty",
      "rdfs:label": {
        "@value": "process classified as",
        "@language": "en"
      },
      "rdfs:domain": {
        "@id": "vf:RecipeProcess"
      },
      "rdfs:range": {
        "@id": "owl:Thing"
      },
      "vs:term_status": "unstable",
      "rdfs:comment": {
        "@value": "References a concept in a common taxonomy or other classification scheme for purposes of categorization or grouping.",
        "@language": "en"
      }
    },
    {
      "@id": "vf:processConformsTo",
      "@type": "owl:ObjectProperty",
      "rdfs:label": {
        "@value": "process conforms to",
        "@language": "en"
      },
      "rdfs:domain": {
        "@id": "vf:RecipeProcess"
      },
      "rdfs:range": {
        "@id": "vf:ProcessSpecification"
      },
      "vs:term_status": "testing",
      "rdfs:comment": {
        "@value": "The standard specification or definition of a process.",
        "@language": "en"
      }
    },
    {
      "@id": "vf:resourceConformsTo",
      "@type": "owl:ObjectProperty",
      "rdfs:label": {
        "@value": "resource conforms to",
        "@language": "en"
      },
      "rdfs:domain": {
        "owl:unionOf": {
          "@list": [
            {
              "@id": "vf:Commitment"
            },
            {
              "@id": "vf:Intent"
            },
            {
              "@id": "vf:EconomicEvent"
            },
            {
              "@id": "vf:Claim"
            },
            {
              "@id": "vf:RecipeFlow"
            }
          ]
        }
      },
      "rdfs:range": {
        "@id": "vf:ResourceSpecification"
      },
      "vs:term_status": "stable",
      "rdfs:comment": {
        "@value": "The primary resource specification or definition of an existing or potential economic resource. A resource will have only one, as this specifies exactly what the resource is.",
        "@language": "en"
      }
    },
    {
      "@id": "vf:conformsTo",
      "@type": "owl:ObjectProperty",
      "rdfs:label": {
        "@value": "conforms to",
        "@language": "en"
      },
      "rdfs:domain": {
        "@id": "vf:EconomicResource"
      },
      "rdfs:range": {
        "@id": "vf:ResourceSpecification"
      },
      "vs:term_status": "stable",
      "rdfs:comment": {
        "@value": "The primary resource knowledge specification or definition of an existing or potential resource.",
        "@language": "en"
      }
    },
    {
      "@id": "vf:stage",
      "@type": "owl:ObjectProperty",
      "rdfs:label": {
        "@value": "stage",
        "@language": "en"
      },
      "rdfs:domain": {
        "owl:unionOf": {
          "@list": [
            {
              "@id": "vf:EconomicResource"
            },
            {
              "@id": "vf:Commitment"
            },
            {
              "@id": "vf:RecipeFlow"
            }
          ]
        }
      },
      "rdfs:range": {
        "@id": "vf:ProcessSpecification"
      },
      "vs:term_status": "testing",
      "rdfs:comment": {
        "@value": "References the ProcessSpecification of the last process the economic resource went through. Stage is used when the last process is important for finding proper resources, such as where the publishing process wants only documents that have gone through the editing process.",
        "@language": "en"
      }
    },
    {
      "@id": "vf:state",
      "@type": "owl:ObjectProperty",
      "rdfs:label": {
        "@value": "state",
        "@language": "en"
      },
      "rdfs:domain": {
        "owl:unionOf": {
          "@list": [
            {
              "@id": "vf:EconomicResource"
            },
            {
              "@id": "vf:EconomicEvent"
            },
            {
              "@id": "vf:RecipeFlow"
            },
            {
              "@id": "vf:Commitment"
            }
          ]
        }
      },
      "rdfs:range": {
        "@id": "xsd:string"
      },
      "vs:term_status": "unstable",
      "rdfs:comment": {
        "@value": "The state of the desired economic resource, after coming out of a test or review process.",
        "@language": "en"
      }
    },
    {
      "@id": "vf:refinementOf",
      "@type": "owl:ObjectProperty",
      "rdfs:label": {
        "@value": "refinement of",
        "@language": "en"
      },
      "rdfs:domain": {
        "owl:unionOf": {
          "@list": [
            {
              "@id": "vf:Scenario"
            },
            {
              "@id": "vf:Plan"
            }
          ]
        }
      },
      "rdfs:range": {
        "@id": "vf:Scenario"
      },
      "vs:term_status": "unstable",
      "rdfs:comment": {
        "@value": "This scenario or plan refines another scenario, often as time moves closer or for more detail.",
        "@language": "en"
      }
    },
    {
      "@id": "vf:nestedIn",
      "@type": "owl:ObjectProperty",
      "rdfs:label": {
        "@value": "nested in",
        "@language": "en"
      },
      "rdfs:domain": {
        "@id": "vf:Process"
      },
      "rdfs:range": {
        "@id": "vf:Scenario"
      },
      "vs:term_status": "unstable",
      "rdfs:comment": {
        "@value": "The process with its inputs and outputs is part of the scenario.",
        "@language": "en"
      }
    },
    {
      "@id": "vf:definedAs",
      "@type": "owl:ObjectProperty",
      "rdfs:label": {
        "@value": "defined as",
        "@language": "en"
      },
      "rdfs:domain": {
        "@id": "vf:Scenario"
      },
      "rdfs:range": {
        "@id": "vf:ScenarioDefinition"
      },
      "vs:term_status": "unstable",
      "rdfs:comment": {
        "@value": "The scenario definition for this scenario, for example yearly budget.",
        "@language": "en"
      }
    },
    {
      "@id": "vf:clauseOf",
      "@type": "owl:ObjectProperty",
      "rdfs:label": {
        "@value": "clause of",
        "@language": "en"
      },
      "rdfs:domain": {
        "@id": "vf:Commitment"
      },
      "rdfs:range": {
        "@id": "vf:Agreement"
      },
      "vs:term_status": "testing",
      "rdfs:comment": {
        "@value": "This commitment is a primary part of the agreement.",
        "@language": "en"
      }
    },
    {
      "@id": "vf:reciprocalClauseOf",
      "@type": "owl:ObjectProperty",
      "rdfs:label": {
        "@value": "reciprocal clause of",
        "@language": "en"
      },
      "rdfs:domain": {
        "@id": "vf:Commitment"
      },
      "rdfs:range": {
        "@id": "vf:Agreement"
      },
      "vs:term_status": "testing",
      "rdfs:comment": {
        "@value": "This commitment is a reciprocal part of the agreement.",
        "@language": "en"
      }
    },
    {
      "@id": "vf:stipulates",
      "@type": "owl:ObjectProperty",
      "owl:inverseOf": {
        "@id": "vf:clauseOf"
      },
      "rdfs:label": {
        "@value": "stipulates",
        "@language": "en"
      },
      "rdfs:domain": {
        "@id": "vf:Agreement"
      },
      "rdfs:range": {
        "@id": "vf:Commitment"
      },
      "vs:term_status": "testing",
      "rdfs:comment": {
        "@value": "All the primary commitments that constitute the agreement.",
        "@language": "en"
      }
    },
    {
      "@id": "vf:stipulatesReciprocal",
      "@type": "owl:ObjectProperty",
      "owl:inverseOf": {
        "@id": "vf:reciprocalClauseOf"
      },
      "rdfs:label": {
        "@value": "stipulates reciprocal",
        "@language": "en"
      },
      "rdfs:domain": {
        "@id": "vf:Agreement"
      },
      "rdfs:range": {
        "@id": "vf:Commitment"
      },
      "vs:term_status": "testing",
      "rdfs:comment": {
        "@value": "All the reciprocal commitments that constitute the agreement.",
        "@language": "en"
      }
    },
    {
      "@id": "vf:realizationOf",
      "@type": "owl:ObjectProperty",
      "rdfs:label": {
        "@value": "realization of",
        "@language": "en"
      },
      "rdfs:domain": {
        "@id": "vf:EconomicEvent"
      },
      "rdfs:range": {
        "@id": "vf:Agreement"
      },
      "vs:term_status": "testing",
      "rdfs:comment": {
        "@value": "This non-reciprocal economic event occurs as part of this agreement.",
        "@language": "en"
      }
    },
    {
      "@id": "vf:realizes",
      "@type": "owl:ObjectProperty",
      "owl:inverseOf": {
        "@id": "vf:realizationOf"
      },
      "rdfs:label": {
        "@value": "realizes",
        "@language": "en"
      },
      "rdfs:domain": {
        "@id": "vf:Agreement"
      },
      "rdfs:range": {
        "@id": "vf:EconomicEvent"
      },
      "vs:term_status": "testing",
      "rdfs:comment": {
        "@value": "All the non-reciprocal economic events (with or without commitments) that realize the agreement.",
        "@language": "en"
      }
    },
    {
      "@id": "vf:reciprocalRealizationOf",
      "@type": "owl:ObjectProperty",
      "rdfs:label": {
        "@value": "reciprocal realization of",
        "@language": "en"
      },
      "rdfs:domain": {
        "@id": "vf:EconomicEvent"
      },
      "rdfs:range": {
        "@id": "vf:Agreement"
      },
      "vs:term_status": "testing",
      "rdfs:comment": {
        "@value": "This reciprocal economic event occurs as part of this agreement.",
        "@language": "en"
      }
    },
    {
      "@id": "vf:realizesReciprocal",
      "@type": "owl:ObjectProperty",
      "owl:inverseOf": {
        "@id": "vf:reciprocalRealizationOf"
      },
      "rdfs:label": {
        "@value": "realizes reciprocal",
        "@language": "en"
      },
      "rdfs:domain": {
        "@id": "vf:Agreement"
      },
      "rdfs:range": {
        "@id": "vf:EconomicEvent"
      },
      "vs:term_status": "testing",
      "rdfs:comment": {
        "@value": "All the reciprocal economic events (with or without commitments) that realize the agreement.",
        "@language": "en"
      }
    },
    {
      "@id": "vf:bundledIn",
      "@type": "owl:ObjectProperty",
      "rdfs:label": {
        "@value": "bundled in",
        "@language": "en"
      },
      "rdfs:domain": {
        "@id": "vf:Agreement"
      },
      "rdfs:range": {
        "@id": "vf:AgreementBundle"
      },
      "vs:term_status": "unstable",
      "rdfs:comment": {
        "@value": "This agreement is bundled with other agreements.",
        "@language": "en"
      }
    },
    {
      "@id": "vf:bundles",
      "@type": "owl:ObjectProperty",
      "owl:inverseOf": {
        "@id": "vf:bundledIn"
      },
      "rdfs:label": {
        "@value": "bundles",
        "@language": "en"
      },
      "rdfs:domain": {
        "@id": "vf:AgreementBundle"
      },
      "rdfs:range": {
        "@id": "vf:Agreement"
      },
      "vs:term_status": "unstable",
      "rdfs:comment": {
        "@value": "All the agreements included in this agreement bundle.",
        "@language": "en"
      }
    },
    {
      "@id": "vf:rules",
      "@type": "owl:DataTypeProperty",
      "rdfs:label": {
        "@value": "rules",
        "@language": "en"
      },
      "rdfs:domain": {
        "@id": "vf:Agreement"
      },
      "rdfs:range": {
        "@id": "xsd:anyURI"
      },
      "vs:term_status": "unstable",
      "rdfs:comment": {
        "@value": "The rules or contract that govern this agreement.",
        "@language": "en"
      }
    },
    {
      "@id": "vf:mappableAddress",
      "@type": "owl:DatatypeProperty",
      "rdfs:label": {
        "@value": "mappable address",
        "@language": "en"
      },
      "rdfs:domain": {
        "@id": "geo:SpatialThing"
      },
      "rdfs:range": {
        "@id": "xsd:string"
      },
      "vs:term_status": "unstable",
      "rdfs:comment": {
        "@value": "A textual address that can be mapped using mapping software.",
        "@language": "en"
      }
    },
    {
      "@id": "vf:roleLabel",
      "@type": "owl:DatatypeProperty",
      "rdfs:label": {
        "@value": "role label",
        "@language": "en"
      },
      "rdfs:domain": {
        "@id": "vf:AgentRelationshipRole"
      },
      "rdfs:range": {
        "@id": "xsd:string"
      },
      "vs:term_status": "unstable",
      "rdfs:comment": {
        "@value": "The human readable name of the role, inverse from the object to the subject. For example, 'is member of'.",
        "@language": "en"
      }
    },
    {
      "@id": "vf:inverseRoleLabel",
      "@type": "owl:DatatypeProperty",
      "rdfs:label": {
        "@value": "inverse role label",
        "@language": "en"
      },
      "rdfs:domain": {
        "@id": "vf:AgentRelationshipRole"
      },
      "rdfs:range": {
        "@id": "xsd:string"
      },
      "vs:term_status": "unstable",
      "rdfs:comment": {
        "@value": "The human readable name of the role, inverse from the object to the subject. For example, 'has member'.",
        "@language": "en"
      }
    },
    {
      "@id": "vf:roleBehavior",
      "@type": "owl:ObjectProperty",
      "rdfs:label": {
        "@value": "role behavior",
        "@language": "en"
      },
      "rdfs:domain": {
        "@id": "vf:AgentRelationshipRole"
      },
      "rdfs:range": {
        "@id": "vf:RoleBehavior"
      },
      "vs:term_status": "unstable",
      "rdfs:comment": {
        "@value": "The generalized behavior of this agent relationship role.",
        "@language": "en"
      }
    },
    {
      "@id": "vf:inputOutput",
      "@type": "owl:ObjectProperty",
      "rdfs:domain": {
        "@id": "vf:Action"
      },
      "rdfs:range": {
        "@id": "vf:InputOutput"
      },
      "rdfs:comment": {
        "@value": "Denotes if a process input or output, or not related to a process.",
        "@language": "en"
      },
      "rdfs:label": {
        "@value": "input/output",
        "@language": "en"
      },
      "vs:term_status": "testing"
    },
    {
      "@id": "vf:pairsWith",
      "@type": "owl:ObjectProperty",
      "rdfs:domain": {
        "@id": "vf:Action"
      },
      "rdfs:range": {
        "@id": "vf:Action"
      },
      "rdfs:comment": {
        "@value": "The action that usually affects the same resource as a complement in the same flow.",
        "@language": "en"
      },
      "rdfs:label": {
        "@value": "pairs with",
        "@language": "en"
      },
      "vs:term_status": "testing"
    },
    {
      "@id": "vf:createResource",
      "@type": "owl:ObjectProperty",
      "rdfs:domain": {
        "@id": "vf:Action"
      },
      "rdfs:range": {
        "@id": "vf:CreateResource"
      },
      "rdfs:comment": {
        "@value": "The action can create an economic resource.",
        "@language": "en"
      },
      "rdfs:label": {
        "@value": "can create resource",
        "@language": "en"
      },
      "vs:term_status": "testing"
    },
    {
      "@id": "vf:eventQuantity",
      "@type": "owl:ObjectProperty",
      "rdfs:domain": {
        "@id": "vf:Action"
      },
      "rdfs:range": {
        "@id": "vf:EventQuantity"
      },
      "rdfs:comment": {
        "@value": "The event quantity applicable is resource quantity, effort quantity, or both.",
        "@language": "en"
      },
      "rdfs:label": {
        "@value": "event quantity",
        "@language": "en"
      },
      "vs:term_status": "testing"
    },
    {
      "@id": "vf:accountingEffect",
      "@type": "owl:ObjectProperty",
      "rdfs:domain": {
        "@id": "vf:Action"
      },
      "rdfs:range": {
        "@id": "vf:AccountingEffect"
      },
      "rdfs:comment": {
        "@value": "The increment and/or decrement effect the action will have on the accounting quantity of an inventoried resource.",
        "@language": "en"
      },
      "rdfs:label": {
        "@value": "accounting effect",
        "@language": "en"
      },
      "vs:term_status": "testing"
    },
    {
      "@id": "vf:onhandEffect",
      "@type": "owl:ObjectProperty",
      "rdfs:domain": {
        "@id": "vf:Action"
      },
      "rdfs:range": {
        "@id": "vf:OnhandEffect"
      },
      "rdfs:comment": {
        "@value": "The increment and/or decrement effect the action will have on the onhand quantity of an inventoried resource.",
        "@language": "en"
      },
      "rdfs:label": {
        "@value": "onhand effect",
        "@language": "en"
      },
      "vs:term_status": "testing"
    },
    {
      "@id": "vf:locationEffect",
      "@type": "owl:ObjectProperty",
      "rdfs:domain": {
        "@id": "vf:Action"
      },
      "rdfs:range": {
        "@id": "vf:LocationEffect"
      },
      "rdfs:comment": {
        "@value": "This action can update the current location of an inventoried resource.",
        "@language": "en"
      },
      "rdfs:label": {
        "@value": "location effect",
        "@language": "en"
      },
      "vs:term_status": "testing"
    },
    {
      "@id": "vf:containedEffect",
      "@type": "owl:ObjectProperty",
      "rdfs:domain": {
        "@id": "vf:Action"
      },
      "rdfs:range": {
        "@id": "vf:ContainedEffect"
      },
      "rdfs:comment": {
        "@value": "The contained in resource should be updated or removed.",
        "@language": "en"
      },
      "rdfs:label": {
        "@value": "contained effect",
        "@language": "en"
      },
      "vs:term_status": "testing"
    },
    {
      "@id": "vf:accountableEffect",
      "@type": "owl:ObjectProperty",
      "rdfs:domain": {
        "@id": "vf:Action"
      },
      "rdfs:range": {
        "@id": "vf:AccountableEffect"
      },
      "rdfs:comment": {
        "@value": "The primaryAccountable should be updated to the event receiver, or not.",
        "@language": "en"
      },
      "rdfs:label": {
        "@value": "accountable effect",
        "@language": "en"
      },
      "vs:term_status": "testing"
    },
    {
      "@id": "vf:stageEffect",
      "@type": "owl:ObjectProperty",
      "rdfs:domain": {
        "@id": "vf:Action"
      },
      "rdfs:range": {
        "@id": "vf:StageEffect"
      },
      "rdfs:comment": {
        "@value": "The stage of the inventoried resource should be updated, or not.",
        "@language": "en"
      },
      "rdfs:label": {
        "@value": "stage effect",
        "@language": "en"
      },
      "vs:term_status": "testing"
    },
    {
      "@id": "vf:stateEffect",
      "@type": "owl:ObjectProperty",
      "rdfs:domain": {
        "@id": "vf:Action"
      },
      "rdfs:range": {
        "@id": "vf:StateEffect"
      },
      "rdfs:comment": {
        "@value": "The state of the from or to inventoried resource should be updated, or not.",
        "@language": "en"
      },
      "rdfs:label": {
        "@value": "state effect",
        "@language": "en"
      },
      "vs:term_status": "testing"
    },
    {
      "@id": "vf:accept",
      "@type": [
        "owl:NamedIndividual",
        "vf:Action"
      ],
      "vf:inputOutput": {
        "@id": "vf:input"
      },
      "vf:pairsWith": {
        "@id": "vf:modify"
      },
      "vf:createResource": {
        "@id": "vf:notApplicable"
      },
      "vf:eventQuantity": {
        "@id": "vf:resource"
      },
      "vf:accountingEffect": {
        "@id": "vf:notApplicable"
      },
      "vf:onhandEffect": {
        "@id": "vf:decrement"
      },
      "vf:locationEffect": {
        "@id": "vf:update"
      },
      "vf:containedEffect": {
        "@id": "vf:notApplicable"
      },
      "vf:accountableEffect": {
        "@id": "vf:notApplicable"
      },
      "vf:stageEffect": {
        "@id": "vf:notApplicable"
      },
      "vf:stateEffect": {
        "@id": "vf:update"
      },
      "rdfs:comment": {
        "@value": "In processes like repair or modification or testing, the same resource will appear in the output.",
        "@language": "en"
      },
      "rdfs:label": {
        "@value": "accept",
        "@language": "en"
      },
      "vs:term_status": "testing"
    },
    {
      "@id": "vf:combine",
      "@type": [
        "owl:NamedIndividual",
        "vf:Action"
      ],
      "vf:inputOutput": {
        "@id": "vf:input"
      },
      "vf:pairsWith": {
        "@id": "vf:notApplicable"
      },
      "vf:createResource": {
        "@id": "vf:notApplicable"
      },
      "vf:eventQuantity": {
        "@id": "vf:resource"
      },
      "vf:accountingEffect": {
        "@id": "vf:notApplicable"
      },
      "vf:onhandEffect": {
        "@id": "vf:decrement"
      },
      "vf:locationEffect": {
        "@id": "vf:notApplicable"
      },
      "vf:containedEffect": {
        "@id": "vf:update"
      },
      "vf:accountableEffect": {
        "@id": "vf:notApplicable"
      },
      "vf:stageEffect": {
        "@id": "vf:notApplicable"
      },
      "vf:stateEffect": {
        "@id": "vf:update"
      },
      "rdfs:comment": {
        "@value": "A resource is combined with other resources into a container resource.",
        "@language": "en"
      },
      "rdfs:label": {
        "@value": "combine",
        "@language": "en"
      },
      "vs:term_status": "unstable"
    },
    {
      "@id": "vf:consume",
      "@type": [
        "owl:NamedIndividual",
        "vf:Action"
      ],
      "vf:inputOutput": {
        "@id": "vf:input"
      },
      "vf:pairsWith": {
        "@id": "vf:notApplicable"
      },
      "vf:createResource": {
        "@id": "vf:notApplicable"
      },
      "vf:eventQuantity": {
        "@id": "vf:resource"
      },
      "vf:accountingEffect": {
        "@id": "vf:decrement"
      },
      "vf:onhandEffect": {
        "@id": "vf:decrement"
      },
      "vf:locationEffect": {
        "@id": "vf:notApplicable"
      },
      "vf:containedEffect": {
        "@id": "vf:notApplicable"
      },
      "vf:accountableEffect": {
        "@id": "vf:notApplicable"
      },
      "vf:stageEffect": {
        "@id": "vf:notApplicable"
      },
      "vf:stateEffect": {
        "@id": "vf:update"
      },
      "rdfs:comment": {
        "@value": "For example an ingredient or component composed into the output, after the process the ingredient is gone.",
        "@language": "en"
      },
      "rdfs:label": {
        "@value": "consume",
        "@language": "en"
      },
      "vs:term_status": "testing"
    },
    {
      "@id": "vf:cite",
      "@type": [
        "owl:NamedIndividual",
        "vf:Action"
      ],
      "vf:inputOutput": {
        "@id": "vf:input"
      },
      "vf:pairsWith": {
        "@id": "vf:notApplicable"
      },
      "vf:createResource": {
        "@id": "vf:notApplicable"
      },
      "vf:eventQuantity": {
        "@id": "vf:resource"
      },
      "vf:accountingEffect": {
        "@id": "vf:notApplicable"
      },
      "vf:onhandEffect": {
        "@id": "vf:notApplicable"
      },
      "vf:locationEffect": {
        "@id": "vf:notApplicable"
      },
      "vf:containedEffect": {
        "@id": "vf:notApplicable"
      },
      "vf:accountableEffect": {
        "@id": "vf:notApplicable"
      },
      "vf:stageEffect": {
        "@id": "vf:notApplicable"
      },
      "vf:stateEffect": {
        "@id": "vf:update"
      },
      "rdfs:comment": {
        "@value": "For example a design file, neither used nor consumed, the file remains available at all times.",
        "@language": "en"
      },
      "rdfs:label": {
        "@value": "cite",
        "@language": "en"
      },
      "vs:term_status": "testing"
    },
    {
      "@id": "vf:copy",
      "@type": [
        "owl:NamedIndividual",
        "vf:Action"
      ],
      "vf:inputOutput": {
        "@id": "vf:notApplicable"
      },
      "vf:pairsWith": {
        "@id": "vf:notApplicable"
      },
      "vf:createResource": {
        "@id": "vf:optionalTo"
      },
      "vf:eventQuantity": {
        "@id": "vf:resource"
      },
      "vf:accountingEffect": {
        "@id": "vf:incrementTo"
      },
      "vf:onhandEffect": {
        "@id": "vf:incrementTo"
      },
      "vf:locationEffect": {
        "@id": "vf:new"
      },
      "vf:containedEffect": {
        "@id": "vf:notApplicable"
      },
      "vf:accountableEffect": {
        "@id": "vf:new"
      },
      "vf:stageEffect": {
        "@id": "vf:notApplicable"
      },
      "vf:stateEffect": {
        "@id": "vf:updateTo"
      },
      "rdfs:comment": {
        "@value": "Create a new version of the resource, without any change to the original.",
        "@language": "en"
      },
      "rdfs:label": {
        "@value": "copy",
        "@language": "en"
      },
      "vs:term_status": "unstable"
    },
    {
      "@id": "vf:deliverService",
      "@type": [
        "owl:NamedIndividual",
        "vf:Action"
      ],
      "vf:inputOutput": {
        "@id": "vf:outputInput"
      },
      "vf:pairsWith": {
        "@id": "vf:notApplicable"
      },
      "vf:createResource": {
        "@id": "vf:notApplicable"
      },
      "vf:eventQuantity": {
        "@id": "vf:resource"
      },
      "vf:accountingEffect": {
        "@id": "vf:notApplicable"
      },
      "vf:onhandEffect": {
        "@id": "vf:notApplicable"
      },
      "vf:locationEffect": {
        "@id": "vf:notApplicable"
      },
      "vf:containedEffect": {
        "@id": "vf:notApplicable"
      },
      "vf:accountableEffect": {
        "@id": "vf:notApplicable"
      },
      "vf:stageEffect": {
        "@id": "vf:notApplicable"
      },
      "vf:stateEffect": {
        "@id": "vf:notApplicable"
      },
      "rdfs:comment": {
        "@value": "New service produced and delivered (a service implies that an agent actively receives the service).",
        "@language": "en"
      },
      "rdfs:label": {
        "@value": "deliver service",
        "@language": "en"
      },
      "vs:term_status": "testing"
    },
    {
      "@id": "vf:dropoff",
      "@type": [
        "owl:NamedIndividual",
        "vf:Action"
      ],
      "vf:createResource": {
        "@id": "vf:notApplicable"
      },
      "vf:eventQuantity": {
        "@id": "vf:resource"
      },
      "vf:inputOutput": {
        "@id": "vf:output"
      },
      "vf:pairsWith": {
        "@id": "vf:pickup"
      },
      "vf:accountingEffect": {
        "@id": "vf:notApplicable"
      },
      "vf:onhandEffect": {
        "@id": "vf:notApplicable"
      },
      "vf:locationEffect": {
        "@id": "vf:update"
      },
      "vf:containedEffect": {
        "@id": "vf:notApplicable"
      },
      "vf:accountableEffect": {
        "@id": "vf:notApplicable"
      },
      "vf:stageEffect": {
        "@id": "vf:update"
      },
      "vf:stateEffect": {
        "@id": "vf:update"
      },
      "rdfs:comment": {
        "@value": "Transported resource or person leaves the process; the same resource or person appeared in the input.",
        "@language": "en"
      },
      "rdfs:label": {
        "@value": "dropoff",
        "@language": "en"
      },
      "vs:term_status": "testing"
    },
    {
      "@id": "vf:lower",
      "@type": [
        "owl:NamedIndividual",
        "vf:Action"
      ],
      "vf:inputOutput": {
        "@id": "vf:notApplicable"
      },
      "vf:createResource": {
        "@id": "vf:optional"
      },
      "vf:eventQuantity": {
        "@id": "vf:resource"
      },
      "vf:pairsWith": {
        "@id": "vf:notApplicable"
      },
      "vf:accountingEffect": {
        "@id": "vf:decrement"
      },
      "vf:onhandEffect": {
        "@id": "vf:decrement"
      },
      "vf:locationEffect": {
        "@id": "vf:notApplicable"
      },
      "vf:containedEffect": {
        "@id": "vf:notApplicable"
      },
      "vf:accountableEffect": {
        "@id": "vf:new"
      },
      "vf:stageEffect": {
        "@id": "vf:notApplicable"
      },
      "vf:stateEffect": {
        "@id": "vf:update"
      },
      "rdfs:comment": {
        "@value": "Adjusts a quantity down based on a beginning balance or inventory count.",
        "@language": "en"
      },
      "rdfs:label": {
        "@value": "lower",
        "@language": "en"
      },
      "vs:term_status": "unstable"
    },
    {
      "@id": "vf:modify",
      "@type": [
        "owl:NamedIndividual",
        "vf:Action"
      ],
      "vf:createResource": {
        "@id": "vf:notApplicable"
      },
      "vf:eventQuantity": {
        "@id": "vf:resource"
      },
      "vf:inputOutput": {
        "@id": "vf:output"
      },
      "vf:pairsWith": {
        "@id": "vf:accept"
      },
      "vf:accountingEffect": {
        "@id": "vf:notApplicable"
      },
      "vf:onhandEffect": {
        "@id": "vf:increment"
      },
      "vf:locationEffect": {
        "@id": "vf:update"
      },
      "vf:containedEffect": {
        "@id": "vf:notApplicable"
      },
      "vf:accountableEffect": {
        "@id": "vf:notApplicable"
      },
      "vf:stageEffect": {
        "@id": "vf:update"
      },
      "vf:stateEffect": {
        "@id": "vf:update"
      },
      "rdfs:comment": {
        "@value": "In processes like repair or modification, the same resource will appear in the input.",
        "@language": "en"
      },
      "rdfs:label": {
        "@value": "modify",
        "@language": "en"
      },
      "vs:term_status": "testing"
    },
    {
      "@id": "vf:move",
      "@type": [
        "owl:NamedIndividual",
        "vf:Action"
      ],
      "vf:inputOutput": {
        "@id": "vf:notApplicable"
      },
      "vf:pairsWith": {
        "@id": "vf:notApplicable"
      },
      "vf:createResource": {
        "@id": "vf:optionalTo"
      },
      "vf:eventQuantity": {
        "@id": "vf:resource"
      },
      "vf:accountingEffect": {
        "@id": "vf:decrementIncrement"
      },
      "vf:onhandEffect": {
        "@id": "vf:decrementIncrement"
      },
      "vf:locationEffect": {
        "@id": "vf:updateTo"
      },
      "vf:containedEffect": {
        "@id": "vf:notApplicable"
      },
      "vf:accountableEffect": {
        "@id": "vf:notApplicable"
      },
      "vf:stageEffect": {
        "@id": "vf:notApplicable"
      },
      "vf:stateEffect": {
        "@id": "vf:updateTo"
      },
      "rdfs:comment": {
        "@value": "Change location and possibly identifier, if location is part of the identification, of a resource with no change of agent rights or possession.",
        "@language": "en"
      },
      "rdfs:label": {
        "@value": "move",
        "@language": "en"
      },
      "vs:term_status": "unstable"
    },
    {
      "@id": "vf:pickup",
      "@type": [
        "owl:NamedIndividual",
        "vf:Action"
      ],
      "vf:inputOutput": {
        "@id": "vf:input"
      },
      "vf:pairsWith": {
        "@id": "vf:dropoff"
      },
      "vf:createResource": {
        "@id": "vf:notApplicable"
      },
      "vf:eventQuantity": {
        "@id": "vf:resource"
      },
      "vf:accountingEffect": {
        "@id": "vf:notApplicable"
      },
      "vf:onhandEffect": {
        "@id": "vf:notApplicable"
      },
      "vf:locationEffect": {
        "@id": "vf:update"
      },
      "vf:containedEffect": {
        "@id": "vf:notApplicable"
      },
      "vf:accountableEffect": {
        "@id": "vf:notApplicable"
      },
      "vf:stageEffect": {
        "@id": "vf:notApplicable"
      },
      "vf:stateEffect": {
        "@id": "vf:update"
      },
      "rdfs:comment": {
        "@value": "Transported resource or person enters the process; the same resource will appear in the output.",
        "@language": "en"
      },
      "rdfs:label": {
        "@value": "pickup",
        "@language": "en"
      },
      "vs:term_status": "testing"
    },
    {
      "@id": "vf:produce",
      "@type": [
        "owl:NamedIndividual",
        "vf:Action"
      ],
      "vf:inputOutput": {
        "@id": "vf:output"
      },
      "vf:pairsWith": {
        "@id": "vf:notApplicable"
      },
      "vf:createResource": {
        "@id": "vf:optional"
      },
      "vf:eventQuantity": {
        "@id": "vf:resource"
      },
      "vf:accountingEffect": {
        "@id": "vf:increment"
      },
      "vf:onhandEffect": {
        "@id": "vf:increment"
      },
      "vf:locationEffect": {
        "@id": "vf:new"
      },
      "vf:containedEffect": {
        "@id": "vf:notApplicable"
      },
      "vf:accountableEffect": {
        "@id": "vf:new"
      },
      "vf:stageEffect": {
        "@id": "vf:update"
      },
      "vf:stateEffect": {
        "@id": "vf:update"
      },
      "rdfs:comment": {
        "@value": "New resource was created in that process or an existing stock resource was added to.",
        "@language": "en"
      },
      "rdfs:label": {
        "@value": "produce",
        "@language": "en"
      },
      "vs:term_status": "testing"
    },
    {
      "@id": "vf:raise",
      "@type": [
        "owl:NamedIndividual",
        "vf:Action"
      ],
      "vf:inputOutput": {
        "@id": "vf:notApplicable"
      },
      "vf:pairsWith": {
        "@id": "vf:notApplicable"
      },
      "vf:createResource": {
        "@id": "vf:optional"
      },
      "vf:eventQuantity": {
        "@id": "vf:resource"
      },
      "vf:accountingEffect": {
        "@id": "vf:increment"
      },
      "vf:onhandEffect": {
        "@id": "vf:increment"
      },
      "vf:locationEffect": {
        "@id": "vf:notApplicable"
      },
      "vf:containedEffect": {
        "@id": "vf:notApplicable"
      },
      "vf:accountableEffect": {
        "@id": "vf:new"
      },
      "vf:stageEffect": {
        "@id": "vf:notApplicable"
      },
      "vf:stateEffect": {
        "@id": "vf:update"
      },
      "rdfs:comment": {
        "@value": "Adjusts a quantity up based on a beginning balance or inventory count.",
        "@language": "en"
      },
      "rdfs:label": {
        "@value": "raise",
        "@language": "en"
      },
      "vs:term_status": "unstable"
    },
    {
      "@id": "vf:separate",
      "@type": [
        "owl:NamedIndividual",
        "vf:Action"
      ],
      "vf:inputOutput": {
        "@id": "vf:output"
      },
      "vf:pairsWith": {
        "@id": "vf:notApplicable"
      },
      "vf:createResource": {
        "@id": "vf:notApplicable"
      },
      "vf:eventQuantity": {
        "@id": "vf:resource"
      },
      "vf:accountingEffect": {
        "@id": "vf:notApplicable"
      },
      "vf:onhandEffect": {
        "@id": "vf:increment"
      },
      "vf:locationEffect": {
        "@id": "vf:notApplicable"
      },
      "vf:containedEffect": {
        "@id": "vf:remove"
      },
      "vf:accountableEffect": {
        "@id": "vf:notApplicable"
      },
      "vf:stageEffect": {
        "@id": "vf:update"
      },
      "vf:stateEffect": {
        "@id": "vf:update"
      },
      "rdfs:comment": {
        "@value": "A resource is removed from a container resource.",
        "@language": "en"
      },
      "rdfs:label": {
        "@value": "unpack",
        "@language": "en"
      },
      "vs:term_status": "unstable"
    },
    {
      "@id": "vf:transferAllRights",
      "@type": [
        "owl:NamedIndividual",
        "vf:Action"
      ],
      "vf:inputOutput": {
        "@id": "vf:notApplicable"
      },
      "vf:pairsWith": {
        "@id": "vf:notApplicable"
      },
      "vf:createResource": {
        "@id": "vf:optionalTo"
      },
      "vf:eventQuantity": {
        "@id": "vf:resource"
      },
      "vf:accountingEffect": {
        "@id": "vf:decrementIncrement"
      },
      "vf:onhandEffect": {
        "@id": "vf:notApplicable"
      },
      "vf:locationEffect": {
        "@id": "vf:notApplicable"
      },
      "vf:containedEffect": {
        "@id": "vf:notApplicable"
      },
      "vf:accountableEffect": {
        "@id": "vf:updateTo"
      },
      "vf:stageEffect": {
        "@id": "vf:notApplicable"
      },
      "vf:stateEffect": {
        "@id": "vf:updateTo"
      },
      "rdfs:comment": {
        "@value": "Give full (in the human realm) rights and responsibilities to another agent, without transferring physical custody.",
        "@language": "en"
      },
      "rdfs:label": {
        "@value": "transfer all rights",
        "@language": "en"
      },
      "vs:term_status": "unstable"
    },
    {
      "@id": "vf:transfer",
      "@type": [
        "owl:NamedIndividual",
        "vf:Action"
      ],
      "vf:inputOutput": {
        "@id": "vf:notApplicable"
      },
      "vf:pairsWith": {
        "@id": "vf:notApplicable"
      },
      "vf:createResource": {
        "@id": "vf:optionalTo"
      },
      "vf:eventQuantity": {
        "@id": "vf:resource"
      },
      "vf:accountingEffect": {
        "@id": "vf:decrementIncrement"
      },
      "vf:onhandEffect": {
        "@id": "vf:decrementIncrement"
      },
      "vf:locationEffect": {
        "@id": "vf:updateTo"
      },
      "vf:containedEffect": {
        "@id": "vf:notApplicable"
      },
      "vf:accountableEffect": {
        "@id": "vf:updateTo"
      },
      "vf:stageEffect": {
        "@id": "vf:notApplicable"
      },
      "vf:stateEffect": {
        "@id": "vf:updateTo"
      },
      "rdfs:comment": {
        "@value": "Give full rights and responsibilities plus physical custody.",
        "@language": "en"
      },
      "rdfs:label": {
        "@value": "transfer",
        "@language": "en"
      },
      "vs:term_status": "testing"
    },
    {
      "@id": "vf:transferCustody",
      "@type": [
        "owl:NamedIndividual",
        "vf:Action"
      ],
      "vf:inputOutput": {
        "@id": "vf:notApplicable"
      },
      "vf:pairsWith": {
        "@id": "vf:notApplicable"
      },
      "vf:createResource": {
        "@id": "vf:optionalTo"
      },
      "vf:eventQuantity": {
        "@id": "vf:resource"
      },
      "vf:accountingEffect": {
        "@id": "vf:notApplicable"
      },
      "vf:onhandEffect": {
        "@id": "vf:decrementIncrement"
      },
      "vf:locationEffect": {
        "@id": "vf:updateTo"
      },
      "vf:containedEffect": {
        "@id": "vf:notApplicable"
      },
      "vf:accountableEffect": {
        "@id": "vf:notApplicable"
      },
      "vf:stageEffect": {
        "@id": "vf:notApplicable"
      },
      "vf:stateEffect": {
        "@id": "vf:updateTo"
      },
      "rdfs:comment": {
        "@value": "Give physical custody and control of a resource, without full accounting or ownership rights.",
        "@language": "en"
      },
      "rdfs:label": {
        "@value": "transfer custody",
        "@language": "en"
      },
      "vs:term_status": "unstable"
    },
    {
      "@id": "vf:use",
      "@type": [
        "owl:NamedIndividual",
        "vf:Action"
      ],
      "vf:inputOutput": {
        "@id": "vf:input"
      },
      "vf:pairsWith": {
        "@id": "vf:notApplicable"
      },
      "vf:createResource": {
        "@id": "vf:notApplicable"
      },
      "vf:eventQuantity": {
        "@id": "vf:both"
      },
      "vf:accountingEffect": {
        "@id": "vf:notApplicable"
      },
      "vf:onhandEffect": {
        "@id": "vf:notApplicable"
      },
      "vf:locationEffect": {
        "@id": "vf:notApplicable"
      },
      "vf:containedEffect": {
        "@id": "vf:notApplicable"
      },
      "vf:accountableEffect": {
        "@id": "vf:notApplicable"
      },
      "vf:stageEffect": {
        "@id": "vf:notApplicable"
      },
      "vf:stateEffect": {
        "@id": "vf:update"
      },
      "rdfs:comment": {
        "@value": "For example a tool used in process; after the process, the tool still exists.",
        "@language": "en"
      },
      "rdfs:label": {
        "@value": "use",
        "@language": "en"
      },
      "vs:term_status": "testing"
    },
    {
      "@id": "vf:work",
      "@type": [
        "owl:NamedIndividual",
        "vf:Action"
      ],
      "vf:inputOutput": {
        "@id": "vf:input"
      },
      "vf:pairsWith": {
        "@id": "vf:notApplicable"
      },
      "vf:createResource": {
        "@id": "vf:notApplicable"
      },
      "vf:eventQuantity": {
        "@id": "vf:effort"
      },
      "vf:accountingEffect": {
        "@id": "vf:notApplicable"
      },
      "vf:onhandEffect": {
        "@id": "vf:notApplicable"
      },
      "vf:locationEffect": {
        "@id": "vf:notApplicable"
      },
      "vf:containedEffect": {
        "@id": "vf:notApplicable"
      },
      "vf:accountableEffect": {
        "@id": "vf:notApplicable"
      },
      "vf:stageEffect": {
        "@id": "vf:notApplicable"
      },
      "vf:stateEffect": {
        "@id": "vf:notApplicable"
      },
      "rdfs:comment": {
        "@value": "Labor power applied to a process.",
        "@language": "en"
      },
      "rdfs:label": {
        "@value": "work",
        "@language": "en"
      },
      "vs:term_status": "testing"
    },
    {
      "@id": "vf:decrement",
      "@type": [
        "owl:NamedIndividual",
        "vf:AccountingEffect",
        "vf:OnhandEffect"
      ],
      "rdfs:comment": {
        "@value": "The effect is to subtract from the inventoried resource accounting or onhand quantity.",
        "@language": "en"
      },
      "rdfs:label": {
        "@value": "decrement",
        "@language": "en"
      },
      "vs:term_status": "unstable"
    },
    {
      "@id": "vf:decrementIncrement",
      "@type": [
        "owl:NamedIndividual",
        "vf:AccountingEffect",
        "vf:OnhandEffect"
      ],
      "rdfs:comment": {
        "@value": "The effect is to subtract from the 'from' inventoried resource, and add to the 'to' inventoried resource, accounting or onhand quantity.",
        "@language": "en"
      },
      "rdfs:label": {
        "@value": "decrement/increment",
        "@language": "en"
      },
      "vs:term_status": "unstable"
    },
    {
      "@id": "vf:increment",
      "@type": [
        "owl:NamedIndividual",
        "vf:AccountingEffect",
        "vf:OnhandEffect"
      ],
      "rdfs:comment": {
        "@value": "The effect is to add to the inventoried resource accounting or onhand quantity.",
        "@language": "en"
      },
      "rdfs:label": {
        "@value": "increment",
        "@language": "en"
      },
      "vs:term_status": "unstable"
    },
    {
      "@id": "vf:incrementTo",
      "@type": [
        "owl:NamedIndividual",
        "vf:AccountingEffect",
        "vf:OnhandEffect"
      ],
      "rdfs:comment": {
        "@value": "The effect is to add to the to (receiver) inventoried resource accounting or onhand quantity.",
        "@language": "en"
      },
      "rdfs:label": {
        "@value": "increment to",
        "@language": "en"
      },
      "vs:term_status": "unstable"
    },
    {
      "@id": "vf:update",
      "@type": [
        "owl:NamedIndividual",
        "vf:ContainedEffect",
        "vf:StageEffect",
        "vf:StateEffect",
        "vf:LocationEffect"
      ],
      "rdfs:comment": {
        "@value": "The effect is to update the resource in the specified property.",
        "@language": "en"
      },
      "rdfs:label": {
        "@value": "update",
        "@language": "en"
      },
      "vs:term_status": "unstable"
    },
    {
      "@id": "vf:updateTo",
      "@type": [
        "owl:NamedIndividual",
        "vf:ContainedEffect",
        "vf:StateEffect",
        "vf:AccountableEffect",
        "vf:LocationEffect"
      ],
      "rdfs:comment": {
        "@value": "The effect is to update the to resource in the specified property.",
        "@language": "en"
      },
      "rdfs:label": {
        "@value": "update",
        "@language": "en"
      },
      "vs:term_status": "unstable"
    },
    {
      "@id": "vf:remove",
      "@type": [
        "owl:NamedIndividual",
        "vf:ContainedEffect"
      ],
      "rdfs:comment": {
        "@value": "The effect is to remove or nullify the specified property from the resource.",
        "@language": "en"
      },
      "rdfs:label": {
        "@value": "remove",
        "@language": "en"
      },
      "vs:term_status": "unstable"
    },
    {
      "@id": "vf:new",
      "@type": [
        "owl:NamedIndividual",
        "vf:AccountableEffect",
        "vf:LocationEffect"
      ],
      "rdfs:comment": {
        "@value": "The effect applies for a new resource created by the event.",
        "@language": "en"
      },
      "rdfs:label": {
        "@value": "remove",
        "@language": "en"
      },
      "vs:term_status": "unstable"
    },
    {
      "@id": "vf:input",
      "@type": [
        "owl:NamedIndividual",
        "vf:InputOutput"
      ],
      "rdfs:comment": {
        "@value": "This kind of flow can be an input to a process.",
        "@language": "en"
      },
      "rdfs:label": {
        "@value": "input",
        "@language": "en"
      },
      "vs:term_status": "testing"
    },
    {
      "@id": "vf:output",
      "@type": [
        "owl:NamedIndividual",
        "vf:InputOutput"
      ],
      "rdfs:comment": {
        "@value": "This kind of flow can be an output to a process.",
        "@language": "en"
      },
      "rdfs:label": {
        "@value": "output",
        "@language": "en"
      },
      "vs:term_status": "testing"
    },
    {
      "@id": "vf:outputInput",
      "@type": [
        "owl:NamedIndividual",
        "vf:InputOutput"
      ],
      "rdfs:comment": {
        "@value": "This kind of flow can be an output to a process, and at the same time an input to another process.",
        "@language": "en"
      },
      "rdfs:label": {
        "@value": "output input",
        "@language": "en"
      },
      "vs:term_status": "unstable"
    },
    {
      "@id": "vf:resource",
      "@type": [
        "owl:NamedIndividual",
        "vf:EventQuantity"
      ],
      "rdfs:comment": {
        "@value": "This event uses resourceQuantity.",
        "@language": "en"
      },
      "rdfs:label": {
        "@value": "resource",
        "@language": "en"
      },
      "vs:term_status": "unstable"
    },
    {
      "@id": "vf:effort",
      "@type": [
        "owl:NamedIndividual",
        "vf:EventQuantity"
      ],
      "rdfs:comment": {
        "@value": "This event uses effortQuantity.",
        "@language": "en"
      },
      "rdfs:label": {
        "@value": "effort",
        "@language": "en"
      },
      "vs:term_status": "unstable"
    },
    {
      "@id": "vf:both",
      "@type": [
        "owl:NamedIndividual",
        "vf:EventQuantity"
      ],
      "rdfs:comment": {
        "@value": "This event can use resourceQuantity and effortQuantity.",
        "@language": "en"
      },
      "rdfs:label": {
        "@value": "both",
        "@language": "en"
      },
      "vs:term_status": "unstable"
    },
    {
      "@id": "vf:optional",
      "@type": [
        "owl:NamedIndividual",
        "vf:CreateResource"
      ],
      "rdfs:comment": {
        "@value": "This kind of flow gives the user the option to create a new resource using resourceInventoriedAs.",
        "@language": "en"
      },
      "rdfs:label": {
        "@value": "optional",
        "@language": "en"
      },
      "vs:term_status": "unstable"
    },
    {
      "@id": "vf:optionalTo",
      "@type": [
        "owl:NamedIndividual",
        "vf:CreateResource"
      ],
      "rdfs:comment": {
        "@value": "This kind of flow gives the user the option to create a new resource using toResourceInventoriedAs.",
        "@language": "en"
      },
      "rdfs:label": {
        "@value": "optional to",
        "@language": "en"
      },
      "vs:term_status": "unstable"
    },
    {
      "@id": "vf:notApplicable",
      "@type": [
        "owl:NamedIndividual",
        "vf:InputOutput",
        "vf:PairsWith",
        "vf:LocationEffect",
        "vf:CreateResource",
        "vf:ContainedEffect"
      ],
      "rdfs:comment": {
        "@value": "This property is not applicable to this kind of flow.",
        "@language": "en"
      },
      "rdfs:label": {
        "@value": "not applicable",
        "@language": "en"
      },
      "vs:term_status": "unstable"
    },
    {
      "@id": "vf:member",
      "@type": [
        "owl:NamedIndividual",
        "vf:RoleBehavior"
      ],
      "rdfs:comment": {
        "@value": "The role is a member type role in relation to an organization.  An agent can be a member of many organizations.",
        "@language": "en"
      },
      "rdfs:label": {
        "@value": "member",
        "@language": "en"
      },
      "vs:term_status": "testing"
    },
    {
      "@id": "vf:subOrganization",
      "@type": [
        "owl:NamedIndividual",
        "vf:RoleBehavior"
      ],
      "rdfs:comment": {
        "@value": "The role is a sub-organization type role in relation to an organization. An agent can be a sub-organization of no more than one organization.",
        "@language": "en"
      },
      "rdfs:label": {
        "@value": "sub-organization",
        "@language": "en"
      },
      "vs:term_status": "testing"
    },
    {
      "@id": "vf:peer",
      "@type": [
        "owl:NamedIndividual",
        "vf:RoleBehavior"
      ],
      "rdfs:comment": {
        "@value": "The role is a peer type role in relation to an agent. Examples are trading partners or mentors.",
        "@language": "en"
      },
      "rdfs:label": {
        "@value": "peer",
        "@language": "en"
      },
      "vs:term_status": "unstable"
    },
    {
      "@id": "vf:offer",
      "@type": [
        "owl:NamedIndividual",
        "vf:ProposalPurpose"
      ],
      "rdfs:comment": {
        "@value": "The proposal is an offer.",
        "@language": "en"
      },
      "rdfs:label": {
        "@value": "offer",
        "@language": "en"
      },
      "vs:term_status": "unstable"
    },
    {
      "@id": "vf:request",
      "@type": [
        "owl:NamedIndividual",
        "vf:ProposalPurpose"
      ],
      "rdfs:comment": {
        "@value": "The proposal is a published request, need, want.",
        "@language": "en"
      },
      "rdfs:label": {
        "@value": "request",
        "@language": "en"
      },
      "vs:term_status": "unstable"
    }
  ]
}
